cfrontend/Cstrategy.v
@@ -65,7 +65,7 @@ Fixpoint simple (a: expr) : bool :=
   | Eassign _ _ _ => false
   | Eassignop _ _ _ _ _ => false
   | Epostincr _ _ _ => false
-  | Ecomma _ _ _ => false
+  | Ecomma _ _ _ _ => false
   | Ecall _ _ _ => false
   | Ebuiltin _ _ _ _ => false
   | Eparen _ _ => false
@@ -83,6 +83,7 @@ Section SIMPLE_EXPRS.
 
 Variable e: env.
 Variable m: mem.
+Variable sq: seqs.
 
 Inductive eval_simple_lvalue: expr -> block -> int -> Prop :=
   | esl_loc: forall b ofs ty,
@@ -112,7 +113,7 @@ with eval_simple_rvalue: expr -> val -> Prop :=
   | esr_rvalof: forall b ofs l ty v,
       eval_simple_lvalue l b ofs ->
       ty = typeof l -> type_is_volatile ty = false ->
-      deref_loc ge ty m b ofs E0 v ->
+      deref_loc ge ty m sq b ofs E0 v ->
       eval_simple_rvalue (Evalof l ty) v
   | esr_addrof: forall b ofs l ty,
       eval_simple_lvalue l b ofs ->
@@ -197,8 +198,8 @@ Inductive leftcontext: kind -> kind -> (expr -> expr) -> Prop :=
   | lctx_builtin: forall k C ef tyargs ty,
       leftcontextlist k C ->
       leftcontext k RV (fun x => Ebuiltin ef tyargs (C x) ty)
-  | lctx_comma: forall k C e2 ty,
-      leftcontext k RV C -> leftcontext k RV (fun x => Ecomma (C x) e2 ty)
+  | lctx_comma: forall k C sp e2 ty,
+      leftcontext k RV C -> leftcontext k RV (fun x => Ecomma sp (C x) e2 ty)
   | lctx_paren: forall k C ty,
       leftcontext k RV C -> leftcontext k RV (fun x => Eparen (C x) ty)
 
@@ -228,152 +229,152 @@ Hint Resolve leftcontext_context.
 
 Inductive estep: state -> trace -> state -> Prop :=
 
-  | step_expr: forall f r k e m v ty,
-      eval_simple_rvalue e m r v ->
+  | step_expr: forall f r k e m sq v ty,
+      eval_simple_rvalue e m sq r v ->
       match r with Eval _ _ => False | _ => True end ->
       ty = typeof r ->
-      estep (ExprState f r k e m)
-         E0 (ExprState f (Eval v ty) k e m)
+      estep (ExprState f r k e m sq)
+         E0 (ExprState f (Eval v ty) k e m sq)
 
-  | step_rvalof_volatile: forall f C l ty k e m b ofs t v,
+  | step_rvalof_volatile: forall f C l ty k e m sq b ofs t v,
       leftcontext RV RV C ->
-      eval_simple_lvalue e m l b ofs ->
-      deref_loc ge ty m b ofs t v ->
+      eval_simple_lvalue e m sq l b ofs ->
+      deref_loc ge ty m sq b ofs t v ->
       ty = typeof l -> type_is_volatile ty = true ->
-      estep (ExprState f (C (Evalof l ty)) k e m)
-          t (ExprState f (C (Eval v ty)) k e m)
+      estep (ExprState f (C (Evalof l ty)) k e m sq)
+          t (ExprState f (C (Eval v ty)) k e m sq)
 
-  | step_seqand_true: forall f C r1 r2 ty k e m v,
+  | step_seqand_true: forall f C r1 r2 ty k e m sq v,
       leftcontext RV RV C ->
-      eval_simple_rvalue e m r1 v ->
+      eval_simple_rvalue e m sq r1 v ->
       bool_val v (typeof r1) = Some true ->
-      estep (ExprState f (C (Eseqand r1 r2 ty)) k e m)
-         E0 (ExprState f (C (Eparen (Eparen r2 type_bool) ty)) k e m)
-  | step_seqand_false: forall f C r1 r2 ty k e m v,
+      estep (ExprState f (C (Eseqand r1 r2 ty)) k e m sq)
+         E0 (ExprState f (C (Eparen (Eparen r2 type_bool) ty)) k e m empty_seqs)
+  | step_seqand_false: forall f C r1 r2 ty k e m sq v,
       leftcontext RV RV C ->
-      eval_simple_rvalue e m r1 v ->
+      eval_simple_rvalue e m sq r1 v ->
       bool_val v (typeof r1) = Some false ->
-      estep (ExprState f (C (Eseqand r1 r2 ty)) k e m)
-         E0 (ExprState f (C (Eval (Vint Int.zero) ty)) k e m)
+      estep (ExprState f (C (Eseqand r1 r2 ty)) k e m sq)
+         E0 (ExprState f (C (Eval (Vint Int.zero) ty)) k e m sq)
 
-  | step_seqor_true: forall f C r1 r2 ty k e m v,
+  | step_seqor_true: forall f C r1 r2 ty k e m sq v,
       leftcontext RV RV C ->
-      eval_simple_rvalue e m r1 v ->
+      eval_simple_rvalue e m sq r1 v ->
       bool_val v (typeof r1) = Some true ->
-      estep (ExprState f (C (Eseqor r1 r2 ty)) k e m)
-         E0 (ExprState f (C (Eval (Vint Int.one) ty)) k e m)
-  | step_seqor_false: forall f C r1 r2 ty k e m v,
+      estep (ExprState f (C (Eseqor r1 r2 ty)) k e m sq)
+         E0 (ExprState f (C (Eval (Vint Int.one) ty)) k e m sq)
+  | step_seqor_false: forall f C r1 r2 ty k e m sq v,
       leftcontext RV RV C ->
-      eval_simple_rvalue e m r1 v ->
+      eval_simple_rvalue e m sq r1 v ->
       bool_val v (typeof r1) = Some false ->
-      estep (ExprState f (C (Eseqor r1 r2 ty)) k e m)
-         E0 (ExprState f (C (Eparen (Eparen r2 type_bool) ty)) k e m)
+      estep (ExprState f (C (Eseqor r1 r2 ty)) k e m sq)
+         E0 (ExprState f (C (Eparen (Eparen r2 type_bool) ty)) k e m empty_seqs)
 
-  | step_condition: forall f C r1 r2 r3 ty k e m v b,
+  | step_condition: forall f C r1 r2 r3 ty k e m sq v b,
       leftcontext RV RV C ->
-      eval_simple_rvalue e m r1 v ->
+      eval_simple_rvalue e m sq r1 v ->
       bool_val v (typeof r1) = Some b ->
-      estep (ExprState f (C (Econdition r1 r2 r3 ty)) k e m)
-         E0 (ExprState f (C (Eparen (if b then r2 else r3) ty)) k e m)
+      estep (ExprState f (C (Econdition r1 r2 r3 ty)) k e m sq)
+         E0 (ExprState f (C (Eparen (if b then r2 else r3) ty)) k e m empty_seqs)
 
-  | step_assign: forall f C l r ty k e m b ofs v v' t m',
+  | step_assign: forall f C l r ty k e m sq b ofs v v' t m' sq',
       leftcontext RV RV C ->
-      eval_simple_lvalue e m l b ofs ->
-      eval_simple_rvalue e m r v ->
+      eval_simple_lvalue e m sq l b ofs ->
+      eval_simple_rvalue e m sq r v ->
       sem_cast v (typeof r) (typeof l) = Some v' ->
-      assign_loc ge (typeof l) m b ofs v' t m' ->
+      assign_loc ge (typeof l) m sq b ofs v' t m' sq' ->
       ty = typeof l ->
-      estep (ExprState f (C (Eassign l r ty)) k e m)
-          t (ExprState f (C (Eval v' ty)) k e m')
+      estep (ExprState f (C (Eassign l r ty)) k e m sq)
+          t (ExprState f (C (Eval v' ty)) k e m' sq')
 
-  | step_assignop: forall f C op l r tyres ty k e m b ofs v1 v2 v3 v4 t1 t2 m' t,
+  | step_assignop: forall f C op l r tyres ty k e m sq b ofs v1 v2 v3 v4 t1 t2 m' sq' t,
       leftcontext RV RV C ->
-      eval_simple_lvalue e m l b ofs ->
-      deref_loc ge (typeof l) m b ofs t1 v1 ->
-      eval_simple_rvalue e m r v2 ->
+      eval_simple_lvalue e m sq l b ofs ->
+      deref_loc ge (typeof l) m sq b ofs t1 v1 ->
+      eval_simple_rvalue e m sq r v2 ->
       sem_binary_operation op v1 (typeof l) v2 (typeof r) m = Some v3 ->
       sem_cast v3 tyres (typeof l) = Some v4 ->
-      assign_loc ge (typeof l) m b ofs v4 t2 m' ->
+      assign_loc ge (typeof l) m sq b ofs v4 t2 m' sq' ->
       ty = typeof l ->
       t = t1 ** t2 ->
-      estep (ExprState f (C (Eassignop op l r tyres ty)) k e m)
-          t (ExprState f (C (Eval v4 ty)) k e m')
+      estep (ExprState f (C (Eassignop op l r tyres ty)) k e m sq)
+          t (ExprState f (C (Eval v4 ty)) k e m' sq')
 
-  | step_assignop_stuck: forall f C op l r tyres ty k e m b ofs v1 v2 t,
+  | step_assignop_stuck: forall f C op l r tyres ty k e m sq b ofs v1 v2 t,
       leftcontext RV RV C ->
-      eval_simple_lvalue e m l b ofs ->
-      deref_loc ge (typeof l) m b ofs t v1 ->
-      eval_simple_rvalue e m r v2 ->
+      eval_simple_lvalue e m sq l b ofs ->
+      deref_loc ge (typeof l) m sq b ofs t v1 ->
+      eval_simple_rvalue e m sq r v2 ->
       match sem_binary_operation op v1 (typeof l) v2 (typeof r) m with
       | None => True
       | Some v3 =>
           match sem_cast v3 tyres (typeof l) with
           | None => True
-          | Some v4 => forall t2 m', ~(assign_loc ge (typeof l) m b ofs v4 t2 m')
+          | Some v4 => forall t2 m' sq', ~(assign_loc ge (typeof l) m sq b ofs v4 t2 m' sq')
           end
       end ->
       ty = typeof l ->
-      estep (ExprState f (C (Eassignop op l r tyres ty)) k e m)
+      estep (ExprState f (C (Eassignop op l r tyres ty)) k e m sq)
           t Stuckstate
 
-  | step_postincr: forall f C id l ty k e m b ofs v1 v2 v3 t1 t2 m' t,
+  | step_postincr: forall f C id l ty k e m sq b ofs v1 v2 v3 t1 t2 m' sq' t,
       leftcontext RV RV C ->
-      eval_simple_lvalue e m l b ofs ->
-      deref_loc ge ty m b ofs t1 v1 ->
+      eval_simple_lvalue e m sq l b ofs ->
+      deref_loc ge ty m sq b ofs t1 v1 ->
       sem_incrdecr id v1 ty = Some v2 ->
       sem_cast v2 (typeconv ty) ty = Some v3 ->
-      assign_loc ge ty m b ofs v3 t2 m' ->
+      assign_loc ge ty m sq b ofs v3 t2 m' sq' ->
       ty = typeof l ->
       t = t1 ** t2 ->
-      estep (ExprState f (C (Epostincr id l ty)) k e m)
-          t (ExprState f (C (Eval v1 ty)) k e m')
+      estep (ExprState f (C (Epostincr id l ty)) k e m sq)
+          t (ExprState f (C (Eval v1 ty)) k e m' sq')
 
-  | step_postincr_stuck: forall f C id l ty k e m b ofs v1 t,
+  | step_postincr_stuck: forall f C id l ty k e m sq b ofs v1 t,
       leftcontext RV RV C ->
-      eval_simple_lvalue e m l b ofs ->
-      deref_loc ge ty m b ofs t v1 ->
+      eval_simple_lvalue e m sq l b ofs ->
+      deref_loc ge ty m sq b ofs t v1 ->
       match sem_incrdecr id v1 ty with
       | None => True
       | Some v2 =>
           match sem_cast v2 (typeconv ty) ty with
           | None => True
-          | Some v3 => forall t2 m', ~(assign_loc ge (typeof l) m b ofs v3 t2 m')
+          | Some v3 => forall t2 m' sq', ~(assign_loc ge (typeof l) m sq b ofs v3 t2 m' sq')
           end
       end ->
       ty = typeof l ->
-      estep (ExprState f (C (Epostincr id l ty)) k e m)
+      estep (ExprState f (C (Epostincr id l ty)) k e m sq)
           t Stuckstate
 
-  | step_comma: forall f C r1 r2 ty k e m v,
+  | step_comma: forall f C sp r1 r2 ty k e m sq v,
       leftcontext RV RV C ->
-      eval_simple_rvalue e m r1 v ->
+      eval_simple_rvalue e m sq r1 v ->
       ty = typeof r2 ->
-      estep (ExprState f (C (Ecomma r1 r2 ty)) k e m)
-         E0 (ExprState f (C r2) k e m)
+      estep (ExprState f (C (Ecomma sp r1 r2 ty)) k e m sq)
+         E0 (ExprState f (C r2) k e m (if sp then empty_seqs else sq))
 
-  | step_paren: forall f C r ty k e m v1 v,
+  | step_paren: forall f C r ty k e m sq v1 v,
       leftcontext RV RV C ->
-      eval_simple_rvalue e m r v1 ->
+      eval_simple_rvalue e m sq r v1 ->
       sem_cast v1 (typeof r) ty = Some v ->
-      estep (ExprState f (C (Eparen r ty)) k e m)
-         E0 (ExprState f (C (Eval v ty)) k e m)
+      estep (ExprState f (C (Eparen r ty)) k e m sq)
+         E0 (ExprState f (C (Eval v ty)) k e m sq)
 
-  | step_call: forall f C rf rargs ty k e m targs tres cconv vf vargs fd,
+  | step_call: forall f C rf rargs ty k e m sq targs tres cconv vf vargs fd,
       leftcontext RV RV C ->
       classify_fun (typeof rf) = fun_case_f targs tres cconv ->
-      eval_simple_rvalue e m rf vf ->
-      eval_simple_list e m rargs targs vargs ->
+      eval_simple_rvalue e m sq rf vf ->
+      eval_simple_list e m sq rargs targs vargs ->
       Genv.find_funct ge vf = Some fd ->
       type_of_fundef fd = Tfunction targs tres cconv ->
-      estep (ExprState f (C (Ecall rf rargs ty)) k e m)
+      estep (ExprState f (C (Ecall rf rargs ty)) k e m sq)
          E0 (Callstate fd vargs (Kcall f e C ty k) m)
 
-  | step_builtin: forall f C ef tyargs rargs ty k e m vargs t vres m',
+  | step_builtin: forall f C ef tyargs rargs ty k e m sq vargs t vres m',
       leftcontext RV RV C ->
-      eval_simple_list e m rargs tyargs vargs ->
+      eval_simple_list e m sq rargs tyargs vargs ->
       external_call ef ge vargs m t vres m' ->
-      estep (ExprState f (C (Ebuiltin ef tyargs rargs ty)) k e m)
-          t (ExprState f (C (Eval vres ty)) k e m').
+      estep (ExprState f (C (Ebuiltin ef tyargs rargs ty)) k e m sq)
+          t (ExprState f (C (Eval vres ty)) k e m' empty_seqs).
 
 Definition step (S: state) (t: trace) (S': state) : Prop :=
   estep S t S' \/ sstep ge S t S'.
@@ -433,12 +434,12 @@ Qed.
 Require Import Classical. 
 
 Lemma safe_imm_safe:
-  forall f C a k e m K,
-  safe (ExprState f (C a) k e m) ->
+  forall f C a k e m sq K,
+  safe (ExprState f (C a) k e m sq) ->
   context K RV C ->
-  imm_safe ge e K a m.
+  imm_safe ge e K a m sq.
 Proof.
-  intros. destruct (classic (imm_safe ge e K a m)); auto.
+  intros. destruct (classic (imm_safe ge e K a m sq)); auto.
   destruct (H Stuckstate). 
   apply star_one. left. econstructor; eauto.
   destruct H2 as [r F]. inv F. 
@@ -463,7 +464,7 @@ Proof.
 Qed.
 
 Lemma rred_kind:
-  forall a m t a' m', rred ge a m t a' m' -> expr_kind a = RV.
+  forall a m sq t a' m' sq', rred ge a m sq t a' m' sq' -> expr_kind a = RV.
 Proof.
   induction 1; auto.
 Qed.
@@ -481,7 +482,7 @@ Proof.
 Qed.
 
 Lemma imm_safe_kind:
-  forall e k a m, imm_safe ge e k a m -> expr_kind a = k.
+  forall e k a m sq, imm_safe ge e k a m sq -> expr_kind a = k.
 Proof.
   induction 1.
   auto.
@@ -492,9 +493,9 @@ Proof.
 Qed.
 
 Lemma safe_expr_kind:
-  forall from C f a k e m,
+  forall from C f a k e m sq,
   context from RV C ->
-  safe (ExprState f (C a) k e m) ->
+  safe (ExprState f (C a) k e m sq) ->
   expr_kind a = from.
 Proof.
   intros. eapply imm_safe_kind. eapply safe_imm_safe; eauto.
@@ -513,7 +514,7 @@ Fixpoint exprlist_all_values (rl: exprlist) : Prop :=
   | Econs _ _ => False
   end.
 
-Definition invert_expr_prop (a: expr) (m: mem) : Prop :=
+Definition invert_expr_prop (a: expr) (m: mem) (sq: seqs) : Prop :=
   match a with
   | Eloc b ofs ty => False
   | Evar x ty =>
@@ -531,7 +532,7 @@ Definition invert_expr_prop (a: expr) (m: mem) : Prop :=
       end
   | Eval v ty => False
   | Evalof (Eloc b ofs ty') ty =>
-      ty' = ty /\ exists t, exists v, deref_loc ge ty m b ofs t v
+      ty' = ty /\ exists t, exists v, deref_loc ge ty m sq b ofs t v
   | Eunop op (Eval v1 ty1) ty =>
       exists v, sem_unary_operation op v1 ty1 = Some v
   | Ebinop op (Eval v1 ty1) (Eval v2 ty2) ty =>
@@ -545,17 +546,17 @@ Definition invert_expr_prop (a: expr) (m: mem) : Prop :=
   | Econdition (Eval v1 ty1) r1 r2 ty =>
       exists b, bool_val v1 ty1 = Some b
   | Eassign (Eloc b ofs ty1) (Eval v2 ty2) ty =>
-      exists v, exists m', exists t,
-      ty = ty1 /\ sem_cast v2 ty2 ty1 = Some v /\ assign_loc ge ty1 m b ofs v t m'
+      exists v, exists m', exists sq', exists t,
+      ty = ty1 /\ sem_cast v2 ty2 ty1 = Some v /\ assign_loc ge ty1 m sq b ofs v t m' sq'
   | Eassignop op (Eloc b ofs ty1) (Eval v2 ty2) tyres ty =>
       exists t, exists v1,
       ty = ty1
-      /\ deref_loc ge ty1 m b ofs t v1
+      /\ deref_loc ge ty1 m sq b ofs t v1
   | Epostincr id (Eloc b ofs ty1) ty =>
       exists t, exists v1,
       ty = ty1
-      /\ deref_loc ge ty m b ofs t v1
-  | Ecomma (Eval v ty1) r2 ty =>
+      /\ deref_loc ge ty m sq b ofs t v1
+  | Ecomma _ (Eval v ty1) r2 ty =>
       typeof r2 = ty
   | Eparen (Eval v1 ty1) ty =>
       exists v, sem_cast v1 ty1 ty = Some v
@@ -575,7 +576,7 @@ Definition invert_expr_prop (a: expr) (m: mem) : Prop :=
   end.
 
 Lemma lred_invert:
-  forall l m l' m', lred ge e l m l' m' -> invert_expr_prop l m.
+  forall l m sq l' m', lred ge e l m l' m' -> invert_expr_prop l m sq.
 Proof.
   induction 1; red; auto.
   exists b; auto.
@@ -586,7 +587,7 @@ Proof.
 Qed.
 
 Lemma rred_invert:
-  forall r m t r' m', rred ge r m t r' m' -> invert_expr_prop r m.
+  forall r m sq t r' m' sq', rred ge r m sq t r' m' sq' -> invert_expr_prop r m sq.
 Proof.
   induction 1; red; auto.
   split; auto; exists t; exists v; auto.
@@ -596,7 +597,7 @@ Proof.
   exists true; auto. exists false; auto.
   exists true; auto. exists false; auto.
   exists b; auto.
-  exists v; exists m'; exists t; auto.
+  exists v; exists m'; exists sq'; exists t; auto.
   exists t; exists v1; auto.
   exists t; exists v1; auto.
   exists v; auto.
@@ -604,9 +605,9 @@ Proof.
 Qed.
 
 Lemma callred_invert:
-  forall r fd args ty m,
+  forall r fd args ty m sq,
   callred ge r fd args ty ->
-  invert_expr_prop r m.
+  invert_expr_prop r m sq.
 Proof.
   intros. inv H. simpl.
   intros. exists tyargs, tyres, cconv, fd, args; auto.
@@ -618,12 +619,12 @@ Combined Scheme context_contextlist_ind from context_ind2, contextlist_ind2.
 
 Lemma invert_expr_context:
   (forall from to C, context from to C ->
-   forall a m,
-   invert_expr_prop a m ->
-   invert_expr_prop (C a) m)
+   forall a m sq,
+   invert_expr_prop a m sq ->
+   invert_expr_prop (C a) m sq)
 /\(forall from C, contextlist from C ->
-  forall a m,
-  invert_expr_prop a m ->
+  forall a m sq,
+  invert_expr_prop a m sq ->
   ~exprlist_all_values (C a)).
 Proof.
   apply context_contextlist_ind; intros; try (exploit H0; [eauto|intros]); simpl.
@@ -645,46 +646,46 @@ Proof.
   destruct e1; auto; destruct (C a); auto; contradiction.
   destruct (C a); auto; contradiction.
   destruct (C a); auto; contradiction.
-  destruct e1; auto. intros. elim (H0 a m); auto.
-  intros. elim (H0 a m); auto. 
+  destruct e1; auto. intros. elim (H0 a m sq); auto.
+  intros. elim (H0 a m sq); auto. 
   destruct (C a); auto; contradiction.
   destruct (C a); auto; contradiction.
   red; intros. destruct (C a); auto. 
-  red; intros. destruct e1; auto. elim (H0 a m); auto. 
+  red; intros. destruct e1; auto. elim (H0 a m sq); auto. 
 Qed.
 
 Lemma imm_safe_inv:
-  forall k a m,
-  imm_safe ge e k a m ->
+  forall k a m sq,
+  imm_safe ge e k a m sq ->
   match a with
   | Eloc _ _ _ => True
   | Eval _ _ => True
-  | _ => invert_expr_prop a m
+  | _ => invert_expr_prop a m sq
   end.
 Proof.
   destruct invert_expr_context as [A B].
   intros. inv H. 
   auto.
   auto.
-  assert (invert_expr_prop (C e0) m).
+  assert (invert_expr_prop (C e0) m sq).
     eapply A; eauto. eapply lred_invert; eauto.
   red in H. destruct (C e0); auto; contradiction.
-  assert (invert_expr_prop (C e0) m).
+  assert (invert_expr_prop (C e0) m sq).
     eapply A; eauto. eapply rred_invert; eauto.
   red in H. destruct (C e0); auto; contradiction.
-  assert (invert_expr_prop (C e0) m).
+  assert (invert_expr_prop (C e0) m sq).
     eapply A; eauto. eapply callred_invert; eauto.
   red in H. destruct (C e0); auto; contradiction.
 Qed.
 
 Lemma safe_inv:
-  forall k C f a K m,
-  safe (ExprState f (C a) K e m) ->
+  forall k C f a K m sq,
+  safe (ExprState f (C a) K e m sq) ->
   context k RV C ->
   match a with
   | Eloc _ _ _ => True
   | Eval _ _ => True
-  | _ => invert_expr_prop a m
+  | _ => invert_expr_prop a m sq
   end.
 Proof.
   intros. eapply imm_safe_inv; eauto. eapply safe_imm_safe; eauto.
@@ -700,16 +701,17 @@ Variable f: function.
 Variable k: cont.
 Variable e: env.
 Variable m: mem.
+Variable sq: seqs.
 
 Lemma eval_simple_steps:
-   (forall a v, eval_simple_rvalue e m a v ->
+   (forall a v, eval_simple_rvalue e m sq a v ->
     forall C, context RV RV C ->
-    star Csem.step ge (ExprState f (C a) k e m)
-                  E0 (ExprState f (C (Eval v (typeof a))) k e m))
-/\ (forall a b ofs, eval_simple_lvalue e m a b ofs ->
+    star Csem.step ge (ExprState f (C a) k e m sq)
+                  E0 (ExprState f (C (Eval v (typeof a))) k e m sq))
+/\ (forall a b ofs, eval_simple_lvalue e m sq a b ofs ->
     forall C, context LV RV C ->
-    star Csem.step ge (ExprState f (C a) k e m)
-                  E0 (ExprState f (C (Eloc b ofs (typeof a))) k e m)).
+    star Csem.step ge (ExprState f (C a) k e m sq)
+                  E0 (ExprState f (C (Eloc b ofs (typeof a))) k e m sq)).
 Proof.
 
 Ltac Steps REC C' := eapply star_trans; [apply (REC C'); eauto | idtac | simpl; reflexivity].
@@ -750,61 +752,61 @@ Ltac FinishL := apply star_one; left; apply step_lred; eauto; simpl; try (econst
 Qed.
 
 Lemma eval_simple_rvalue_steps:
-  forall a v, eval_simple_rvalue e m a v ->
+  forall a v, eval_simple_rvalue e m sq a v ->
   forall C, context RV RV C ->
-  star Csem.step ge (ExprState f (C a) k e m)
-                E0 (ExprState f (C (Eval v (typeof a))) k e m).
+  star Csem.step ge (ExprState f (C a) k e m sq)
+                E0 (ExprState f (C (Eval v (typeof a))) k e m sq).
 Proof (proj1 eval_simple_steps).
 
 Lemma eval_simple_lvalue_steps:
-  forall a b ofs, eval_simple_lvalue e m a b ofs ->
+  forall a b ofs, eval_simple_lvalue e m sq a b ofs ->
   forall C, context LV RV C ->
-  star Csem.step ge (ExprState f (C a) k e m)
-                E0 (ExprState f (C (Eloc b ofs (typeof a))) k e m).
+  star Csem.step ge (ExprState f (C a) k e m sq)
+                E0 (ExprState f (C (Eloc b ofs (typeof a))) k e m sq).
 Proof (proj2 eval_simple_steps).
 
 Corollary eval_simple_rvalue_safe:
   forall C a v,
-  eval_simple_rvalue e m a v ->
-  context RV RV C -> safe (ExprState f (C a) k e m) ->
-  safe (ExprState f (C (Eval v (typeof a))) k e m).
+  eval_simple_rvalue e m sq a v ->
+  context RV RV C -> safe (ExprState f (C a) k e m sq) ->
+  safe (ExprState f (C (Eval v (typeof a))) k e m sq).
 Proof.
   intros. eapply safe_steps; eauto. eapply eval_simple_rvalue_steps; eauto.
 Qed.
 
 Corollary eval_simple_lvalue_safe:
   forall C a b ofs,
-  eval_simple_lvalue e m a b ofs ->
-  context LV RV C -> safe (ExprState f (C a) k e m) ->
-  safe (ExprState f (C (Eloc b ofs (typeof a))) k e m).
+  eval_simple_lvalue e m sq a b ofs ->
+  context LV RV C -> safe (ExprState f (C a) k e m sq) ->
+  safe (ExprState f (C (Eloc b ofs (typeof a))) k e m sq).
 Proof.
   intros. eapply safe_steps; eauto. eapply eval_simple_lvalue_steps; eauto.
 Qed.
 
 Lemma simple_can_eval:
   forall a from C,
-  simple a = true -> context from RV C -> safe (ExprState f (C a) k e m) ->
+  simple a = true -> context from RV C -> safe (ExprState f (C a) k e m sq) ->
   match from with
-  | LV => exists b, exists ofs, eval_simple_lvalue e m a b ofs
-  | RV => exists v, eval_simple_rvalue e m a v
+  | LV => exists b, exists ofs, eval_simple_lvalue e m sq a b ofs
+  | RV => exists v, eval_simple_rvalue e m sq a v
   end.
 Proof.
 Ltac StepL REC C' a :=
   let b := fresh "b" in let ofs := fresh "ofs" in
   let E := fresh "E" in let S := fresh "SAFE" in
   exploit (REC LV C'); eauto; intros [b [ofs E]];
-  assert (S: safe (ExprState f (C' (Eloc b ofs (typeof a))) k e m)) by 
+  assert (S: safe (ExprState f (C' (Eloc b ofs (typeof a))) k e m sq)) by 
     (eapply (eval_simple_lvalue_safe C'); eauto);
   simpl in S.
 Ltac StepR REC C' a :=
   let v := fresh "v" in let E := fresh "E" in let S := fresh "SAFE" in
   exploit (REC RV C'); eauto; intros [v E];
-  assert (S: safe (ExprState f (C' (Eval v (typeof a))) k e m)) by 
+  assert (S: safe (ExprState f (C' (Eval v (typeof a))) k e m sq)) by 
     (eapply (eval_simple_rvalue_safe C'); eauto);
   simpl in S.
 
   induction a; intros from C S CTX SAFE;
-  generalize (safe_expr_kind _ _ _ _ _ _ _ CTX SAFE); intro K; subst;
+  generalize (safe_expr_kind _ _ _ _ _ _ _ _ CTX SAFE); intro K; subst;
   simpl in S; try discriminate; simpl.
 (* val *)
   exists v; constructor.
@@ -855,9 +857,9 @@ Qed.
 
 Lemma simple_can_eval_rval:
   forall r C, 
-  simple r = true -> context RV RV C -> safe (ExprState f (C r) k e m) ->
-  exists v, eval_simple_rvalue e m r v
-        /\ safe (ExprState f (C (Eval v (typeof r))) k e m).
+  simple r = true -> context RV RV C -> safe (ExprState f (C r) k e m sq) ->
+  exists v, eval_simple_rvalue e m sq r v
+        /\ safe (ExprState f (C (Eval v (typeof r))) k e m sq).
 Proof.
   intros. exploit (simple_can_eval r RV); eauto. intros [v A]. 
   exists v; split; auto. eapply eval_simple_rvalue_safe; eauto.
@@ -865,9 +867,9 @@ Qed.
 
 Lemma simple_can_eval_lval:
   forall l C, 
-  simple l = true -> context LV RV C -> safe (ExprState f (C l) k e m) ->
-  exists b, exists ofs, eval_simple_lvalue e m l b ofs
-         /\ safe (ExprState f (C (Eloc b ofs (typeof l))) k e m).
+  simple l = true -> context LV RV C -> safe (ExprState f (C l) k e m sq) ->
+  exists b, exists ofs, eval_simple_lvalue e m sq l b ofs
+         /\ safe (ExprState f (C (Eloc b ofs (typeof l))) k e m sq).
 Proof.
   intros. exploit (simple_can_eval l LV); eauto. intros [b [ofs A]]. 
   exists b; exists ofs; split; auto. eapply eval_simple_lvalue_safe; eauto.
@@ -883,13 +885,13 @@ Inductive eval_simple_list': exprlist -> list val -> Prop :=
   | esrl'_nil:
       eval_simple_list' Enil nil
   | esrl'_cons: forall r rl v vl,
-      eval_simple_rvalue e m r v ->
+      eval_simple_rvalue e m sq r v ->
       eval_simple_list' rl vl ->
       eval_simple_list' (Econs r rl) (v :: vl).
 
 Lemma eval_simple_list_implies:
   forall rl tyl vl,
-  eval_simple_list e m rl tyl vl -> 
+  eval_simple_list e m sq rl tyl vl -> 
   exists vl', cast_arguments (rval_list vl' rl) tyl vl /\ eval_simple_list' rl vl'.
 Proof.
   induction 1.
@@ -903,7 +905,7 @@ Lemma can_eval_simple_list:
   eval_simple_list' rl vl ->
   forall tyl vl',
   cast_arguments (rval_list vl rl) tyl vl' ->
-  eval_simple_list e m rl tyl vl'.
+  eval_simple_list e m sq rl tyl vl'.
 Proof.
   induction 1; simpl; intros. 
   inv H. constructor.
@@ -978,8 +980,8 @@ Hint Resolve contextlist'_head contextlist'_tail.
 Lemma eval_simple_list_steps:
   forall rl vl, eval_simple_list' rl vl ->
   forall C, contextlist' C ->
-  star Csem.step ge (ExprState f (C rl) k e m)
-                E0 (ExprState f (C (rval_list vl rl)) k e m).
+  star Csem.step ge (ExprState f (C rl) k e m sq)
+                E0 (ExprState f (C (rval_list vl rl)) k e m sq).
 Proof.
   induction 1; intros. 
 (* nil *)
@@ -995,7 +997,7 @@ Lemma simple_list_can_eval:
   forall rl C,
   simplelist rl = true ->
   contextlist' C ->
-  safe (ExprState f (C rl) k e m) ->
+  safe (ExprState f (C rl) k e m sq) ->
   exists vl, eval_simple_list' rl vl.
 Proof.
   induction rl; intros.
@@ -1026,6 +1028,7 @@ Variable f: function.
 Variable k: cont.
 Variable e: env.
 Variable m: mem.
+Variable sq: seqs.
 
 Definition simple_side_effect (r: expr) : Prop :=
   match r with
@@ -1036,7 +1039,7 @@ Definition simple_side_effect (r: expr) : Prop :=
   | Eassign l1 r2 _ => simple l1 = true /\ simple r2 = true
   | Eassignop _ l1 r2 _ _ => simple l1 = true /\ simple r2 = true
   | Epostincr _ l1 _ => simple l1 = true
-  | Ecomma r1 r2 _ => simple r1 = true
+  | Ecomma _ r1 r2 _ => simple r1 = true
   | Ecall r1 rl _ => simple r1 = true /\ simplelist rl = true
   | Ebuiltin ef tyargs rl _ => simplelist rl = true
   | Eparen r1 _ => simple r1 = true
@@ -1051,11 +1054,11 @@ Hint Constructors leftcontext leftcontextlist.
 
 Lemma decompose_expr:
   (forall a from C,
-   context from RV C -> safe (ExprState f (C a) k e m) ->
+   context from RV C -> safe (ExprState f (C a) k e m sq) ->
        simple a = true
     \/ exists C', exists a', a = C' a' /\ simple_side_effect a' /\ leftcontext RV from C')
 /\(forall rl C,
-   contextlist' C -> safe (ExprState f (C rl) k e m) ->
+   contextlist' C -> safe (ExprState f (C rl) k e m sq) ->
        simplelist rl = true
     \/ exists C', exists a', rl = C' a' /\ simple_side_effect a' /\ leftcontextlist RV C').
 Proof.
@@ -1100,7 +1103,7 @@ Ltac Base :=
 (* postincr *)
   Kind. Rec H LV C (fun x => Epostincr id x ty). Base.
 (* comma *)
-  Kind. Rec H RV C (fun x => Ecomma x r2 ty). Base.
+  Kind. Rec H RV C (fun x => Ecomma sp x r2 ty). Base.
 (* call *)
   Kind. Rec H RV C (fun x => Ecall x rargs ty). 
   destruct (H0 (fun x => C (Ecall r1 x ty))) as [A | [C' [a' [D [A B]]]]].
@@ -1127,7 +1130,7 @@ Qed.
 
 Lemma decompose_topexpr:
   forall a,
-  safe (ExprState f a k e m) ->
+  safe (ExprState f a k e m sq) ->
        simple a = true
     \/ exists C, exists a', a = C a' /\ simple_side_effect a' /\ leftcontext RV RV C.
 Proof.
@@ -1202,7 +1205,7 @@ Proof.
   left; apply step_rred with (C := fun x => C(Eassign (Eloc b ofs (typeof l)) x (typeof l))); eauto. econstructor; eauto.  
   apply star_one. 
   left; eapply step_stuck; eauto.
-  red; intros. exploit imm_safe_inv; eauto. simpl. intros [v4' [m' [t' [A [B D]]]]].
+  red; intros. exploit imm_safe_inv; eauto. simpl. intros [v4' [m' [sq' [t' [A [B D]]]]]].
   rewrite B in H4. eelim H4; eauto.
   reflexivity.
   apply star_one.
@@ -1216,10 +1219,11 @@ Proof.
   eapply plus_left.
   left; apply step_rred; auto. econstructor; eauto.
   eapply star_left.
-  left; apply step_rred with (C := fun x => C (Ecomma (Eassign (Eloc b ofs (typeof l)) x (typeof l)) (Eval v1 (typeof l)) (typeof l))); eauto.
+  left; apply step_rred with (C := fun x =>
+    C (Ecomma false (Eassign (Eloc b ofs (typeof l)) x (typeof l)) (Eval v1 (typeof l)) (typeof l))); eauto.
   econstructor. instantiate (1 := v2). destruct id; assumption. 
   eapply star_left.
-  left; apply step_rred with (C := fun x => C (Ecomma x (Eval v1 (typeof l)) (typeof l))); eauto.
+  left; apply step_rred with (C := fun x => C (Ecomma false x (Eval v1 (typeof l)) (typeof l))); eauto.
   econstructor; eauto.
   apply star_one.
   left; apply step_rred; auto. econstructor; eauto. 
@@ -1235,21 +1239,23 @@ Proof.
     destruct id; auto.
   destruct (sem_incrdecr id v1 (typeof l)) as [v2|].
   eapply star_left.
-  left; apply step_rred with (C := fun x => C (Ecomma (Eassign (Eloc b ofs (typeof l)) x (typeof l)) (Eval v1 (typeof l)) (typeof l))); eauto.
+  left; apply step_rred with (C := fun x =>
+    C (Ecomma false (Eassign (Eloc b ofs (typeof l)) x (typeof l)) (Eval v1 (typeof l)) (typeof l))); eauto.
   econstructor; eauto.
   apply star_one.
-  left; eapply step_stuck with (C := fun x => C (Ecomma x (Eval v1 (typeof l)) (typeof l))); eauto.
-  red; intros. exploit imm_safe_inv; eauto. simpl. intros [v3 [m' [t' [A [B D]]]]].
+  left; eapply step_stuck with (C := fun x => C (Ecomma false x (Eval v1 (typeof l)) (typeof l))); eauto.
+  red; intros. exploit imm_safe_inv; eauto. simpl. intros [v3 [m' [sq' [t' [A [B D]]]]]].
   rewrite B in H3. eelim H3; eauto.
   reflexivity.
   apply star_one.
-  left; eapply step_stuck with (C := fun x => C (Ecomma (Eassign (Eloc b ofs (typeof l)) x (typeof l)) (Eval v1 (typeof l)) (typeof l))); eauto.
+  left; eapply step_stuck with (C := fun x =>
+    C (Ecomma false (Eassign (Eloc b ofs (typeof l)) x (typeof l)) (Eval v1 (typeof l)) (typeof l))); eauto.
   red; intros. exploit imm_safe_inv; eauto. simpl. intros [v2 A]. congruence.
   reflexivity. 
   traceEq.
 (* comma *)
   eapply plus_right.
-  eapply eval_simple_rvalue_steps with (C := fun x => C(Ecomma x r2 (typeof r2))); eauto.
+  eapply eval_simple_rvalue_steps with (C := fun x => C(Ecomma sp x r2 (typeof r2))); eauto.
   left; apply step_rred; eauto. econstructor; eauto. auto.
 (* paren *)
   eapply plus_right; eauto.
@@ -1274,116 +1280,116 @@ Proof.
 Qed.
 
 Lemma can_estep:
-  forall f a k e m,
-  safe (ExprState f a k e m) ->
+  forall f a k e m sq,
+  safe (ExprState f a k e m sq) ->
   match a with Eval _ _ => False | _ => True end ->
-  exists t, exists S, estep (ExprState f a k e m) t S.
+  exists t, exists S, estep (ExprState f a k e m sq) t S.
 Proof.
-  intros. destruct (decompose_topexpr f k e m a H) as [A | [C [b [P [Q R]]]]].
+  intros. destruct (decompose_topexpr f k e m sq a H) as [A | [C [b [P [Q R]]]]].
 (* simple expr *)
-  exploit (simple_can_eval f k e m a RV (fun x => x)); auto. intros [v P].
+  exploit (simple_can_eval f k e m sq a RV (fun x => x)); auto. intros [v P].
   econstructor; econstructor; eapply step_expr; eauto. 
 (* side effect *)
   clear H0. subst a. red in Q. destruct b; try contradiction. 
 (* valof volatile *)
   destruct Q.
-  exploit (simple_can_eval_lval f k e m b (fun x => C(Evalof x ty))); eauto.
+  exploit (simple_can_eval_lval f k e m sq b (fun x => C(Evalof x ty))); eauto.
   intros [b1 [ofs [E1 S1]]].
   exploit safe_inv. eexact S1. eauto. simpl. intros [A [t [v B]]].
   econstructor; econstructor; eapply step_rvalof_volatile; eauto. congruence. 
 (* seqand *)
-  exploit (simple_can_eval_rval f k e m b1 (fun x => C(Eseqand x b2 ty))); eauto.
+  exploit (simple_can_eval_rval f k e m sq b1 (fun x => C(Eseqand x b2 ty))); eauto.
   intros [v1 [E1 S1]].
   exploit safe_inv. eexact S1. eauto. simpl. intros [b BV].
   destruct b.
   econstructor; econstructor; eapply step_seqand_true; eauto. 
   econstructor; econstructor; eapply step_seqand_false; eauto. 
 (* seqor *)
-  exploit (simple_can_eval_rval f k e m b1 (fun x => C(Eseqor x b2 ty))); eauto.
+  exploit (simple_can_eval_rval f k e m sq b1 (fun x => C(Eseqor x b2 ty))); eauto.
   intros [v1 [E1 S1]].
   exploit safe_inv. eexact S1. eauto. simpl. intros [b BV].
   destruct b.
   econstructor; econstructor; eapply step_seqor_true; eauto. 
   econstructor; econstructor; eapply step_seqor_false; eauto. 
 (* condition *)
-  exploit (simple_can_eval_rval f k e m b1 (fun x => C(Econdition x b2 b3 ty))); eauto.
+  exploit (simple_can_eval_rval f k e m sq b1 (fun x => C(Econdition x b2 b3 ty))); eauto.
   intros [v1 [E1 S1]].
   exploit safe_inv. eexact S1. eauto. simpl. intros [b BV].
   econstructor; econstructor. eapply step_condition; eauto. 
 (* assign *)
   destruct Q.
-  exploit (simple_can_eval_lval f k e m b1 (fun x => C(Eassign x b2 ty))); eauto.
+  exploit (simple_can_eval_lval f k e m sq b1 (fun x => C(Eassign x b2 ty))); eauto.
   intros [b [ofs [E1 S1]]].
-  exploit (simple_can_eval_rval f k e m b2 (fun x => C(Eassign (Eloc b ofs (typeof b1)) x ty))); eauto.
+  exploit (simple_can_eval_rval f k e m sq b2 (fun x => C(Eassign (Eloc b ofs (typeof b1)) x ty))); eauto.
   intros [v [E2 S2]].
-  exploit safe_inv. eexact S2. eauto. simpl. intros [v' [m' [t [A [B D]]]]].
+  exploit safe_inv. eexact S2. eauto. simpl. intros [v' [m' [sq' [t [A [B D]]]]]].
   econstructor; econstructor; eapply step_assign; eauto. 
 (* assignop *)
   destruct Q.
-  exploit (simple_can_eval_lval f k e m b1 (fun x => C(Eassignop op x b2 tyres ty))); eauto.
+  exploit (simple_can_eval_lval f k e m sq b1 (fun x => C(Eassignop op x b2 tyres ty))); eauto.
   intros [b [ofs [E1 S1]]].
-  exploit (simple_can_eval_rval f k e m b2 (fun x => C(Eassignop op (Eloc b ofs (typeof b1)) x tyres ty))); eauto.
+  exploit (simple_can_eval_rval f k e m sq b2 (fun x => C(Eassignop op (Eloc b ofs (typeof b1)) x tyres ty))); eauto.
   intros [v [E2 S2]].
   exploit safe_inv. eexact S2. eauto. simpl. intros [t1 [v1 [A B]]].
   destruct (sem_binary_operation op v1 (typeof b1) v (typeof b2) m) as [v3|] eqn:?.
   destruct (sem_cast v3 tyres (typeof b1)) as [v4|] eqn:?.
-  destruct (classic (exists t2, exists m', assign_loc ge (typeof b1) m b ofs v4 t2 m')).
-  destruct H2 as [t2 [m' D]].
+  destruct (classic (exists t2, exists m', exists sq', assign_loc ge (typeof b1) m sq b ofs v4 t2 m' sq')).
+  destruct H2 as [t2 [m' [sq' D]]].
   econstructor; econstructor; eapply step_assignop; eauto.
   econstructor; econstructor; eapply step_assignop_stuck; eauto. 
-  rewrite Heqo. rewrite Heqo0. intros; red; intros. elim H2. exists t2; exists m'; auto.
+  rewrite Heqo. rewrite Heqo0. intros; red; intros. elim H2. exists t2; exists m'; exists sq'; auto.
   econstructor; econstructor; eapply step_assignop_stuck; eauto. 
   rewrite Heqo. rewrite Heqo0. auto.
   econstructor; econstructor; eapply step_assignop_stuck; eauto. 
   rewrite Heqo. auto.
 (* postincr *)
-  exploit (simple_can_eval_lval f k e m b (fun x => C(Epostincr id x ty))); eauto.
+  exploit (simple_can_eval_lval f k e m sq b (fun x => C(Epostincr id x ty))); eauto.
   intros [b1 [ofs [E1 S1]]].
   exploit safe_inv. eexact S1. eauto. simpl. intros [t [v1 [A B]]].
   destruct (sem_incrdecr id v1 ty) as [v2|] eqn:?.
   destruct (sem_cast v2 (typeconv ty) ty) as [v3|] eqn:?.
-  destruct (classic (exists t2, exists m', assign_loc ge ty m b1 ofs v3 t2 m')).
-  destruct H0 as [t2 [m' D]].
+  destruct (classic (exists t2, exists m', exists sq', assign_loc ge ty m sq b1 ofs v3 t2 m' sq')).
+  destruct H0 as [t2 [m' [sq' D]]].
   econstructor; econstructor; eapply step_postincr; eauto.
   econstructor; econstructor; eapply step_postincr_stuck; eauto. 
-  rewrite Heqo. rewrite Heqo0. intros; red; intros. elim H0. exists t2; exists m'; congruence.
+  rewrite Heqo. rewrite Heqo0. intros; red; intros. elim H0. exists t2; exists m'; exists sq'; congruence.
   econstructor; econstructor; eapply step_postincr_stuck; eauto. 
   rewrite Heqo. rewrite Heqo0. auto.
   econstructor; econstructor; eapply step_postincr_stuck; eauto. 
   rewrite Heqo. auto.
 (* comma *)
-  exploit (simple_can_eval_rval f k e m b1 (fun x => C(Ecomma x b2 ty))); eauto.
+  exploit (simple_can_eval_rval f k e m sq b1 (fun x => C(Ecomma sp x b2 ty))); eauto.
   intros [v1 [E1 S1]].
   exploit safe_inv. eexact S1. eauto. simpl. intros EQ.
   econstructor; econstructor; eapply step_comma; eauto.
 (* call *)
   destruct Q.
-  exploit (simple_can_eval_rval f k e m b (fun x => C(Ecall x rargs ty))); eauto.
+  exploit (simple_can_eval_rval f k e m sq b (fun x => C(Ecall x rargs ty))); eauto.
   intros [vf [E1 S1]].
   pose (C' := fun x => C(Ecall (Eval vf (typeof b)) x ty)).
   assert (contextlist' C'). unfold C'; eapply contextlist'_call with (rl0 := Enil); auto.
-  exploit (simple_list_can_eval f k e m rargs C'); eauto.
+  exploit (simple_list_can_eval f k e m sq rargs C'); eauto.
   intros [vl E2].
   exploit safe_inv. 2: eapply leftcontext_context; eexact R.
   eapply safe_steps. eexact S1.
-  apply (eval_simple_list_steps f k e m rargs vl E2 C'); auto.
+  apply (eval_simple_list_steps f k e m sq rargs vl E2 C'); auto.
   simpl. intros X. exploit X. eapply rval_list_all_values. 
   intros [tyargs [tyres [cconv [fd [vargs [P [Q [U V]]]]]]]].
   econstructor; econstructor; eapply step_call; eauto. eapply can_eval_simple_list; eauto. 
 (* builtin *)
   pose (C' := fun x => C(Ebuiltin ef tyargs x ty)).
   assert (contextlist' C'). unfold C'; eapply contextlist'_builtin with (rl0 := Enil); auto.
-  exploit (simple_list_can_eval f k e m rargs C'); eauto.
+  exploit (simple_list_can_eval f k e m sq rargs C'); eauto.
   intros [vl E].
   exploit safe_inv. 2: eapply leftcontext_context; eexact R.
   eapply safe_steps. eexact H.
-  apply (eval_simple_list_steps f k e m rargs vl E C'); auto.
+  apply (eval_simple_list_steps f k e m sq rargs vl E C'); auto.
   simpl. intros X. exploit X. eapply rval_list_all_values.
   intros [vargs [t [vres [m' [U V]]]]].
   econstructor; econstructor; eapply step_builtin; eauto.
   eapply can_eval_simple_list; eauto. 
 (* paren *)
-  exploit (simple_can_eval_rval f k e m b (fun x => C(Eparen x ty))); eauto.
+  exploit (simple_can_eval_rval f k e m sq b (fun x => C(Eparen x ty))); eauto.
   intros [v1 [E1 S1]].
   exploit safe_inv. eexact S1. eauto. simpl. intros [v CAST].
   econstructor; econstructor; eapply step_paren; eauto.
@@ -1436,18 +1442,18 @@ Definition semantics (p: program) :=
 (** This semantics is receptive to changes in events. *)
 
 Remark deref_loc_trace:
-  forall F V (ge: Genv.t F V) ty m b ofs t v,
-  deref_loc ge ty m b ofs t v ->
+  forall F V (ge: Genv.t F V) ty m sq b ofs t v,
+  deref_loc ge ty m sq b ofs t v ->
   match t with nil => True | ev :: nil => True | _ => False end.
 Proof.
   intros. inv H; simpl; auto. inv H2; simpl; auto. 
 Qed.
 
 Remark deref_loc_receptive:
-  forall F V (ge: Genv.t F V) ty m b ofs ev1 t1 v ev2,
-  deref_loc ge ty m b ofs (ev1 :: t1) v ->
+  forall F V (ge: Genv.t F V) ty m sq b ofs ev1 t1 v ev2,
+  deref_loc ge ty m sq b ofs (ev1 :: t1) v ->
   match_traces ge (ev1 :: nil) (ev2 :: nil) ->
-  t1 = nil /\ exists v', deref_loc ge ty m b ofs (ev2 :: nil) v'.
+  t1 = nil /\ exists v', deref_loc ge ty m sq b ofs (ev2 :: nil) v'.
 Proof.
   intros.
   assert (t1 = nil). exploit deref_loc_trace; eauto. destruct t1; simpl; tauto.
@@ -1456,16 +1462,16 @@ Proof.
 Qed.
 
 Remark assign_loc_trace:
-  forall F V (ge: Genv.t F V) ty m b ofs t v m',
-  assign_loc ge ty m b ofs v t m' ->
+  forall F V (ge: Genv.t F V) ty m sq b ofs t v m' sq',
+  assign_loc ge ty m sq b ofs v t m' sq' ->
   match t with nil => True | ev :: nil => output_event ev | _ => False end.
 Proof.
   intros. inv H; simpl; auto. inv H2; simpl; auto. 
 Qed.
 
 Remark assign_loc_receptive:
-  forall F V (ge: Genv.t F V) ty m b ofs ev1 t1 v m' ev2,
-  assign_loc ge ty m b ofs v (ev1 :: t1) m' ->
+  forall F V (ge: Genv.t F V) ty m sq b ofs ev1 t1 v m' sq' ev2,
+  assign_loc ge ty m sq b ofs v (ev1 :: t1) m' sq' ->
   match_traces ge (ev1 :: nil) (ev2 :: nil) ->
   ev1 :: t1 = ev2 :: nil.
 Proof.
@@ -1494,11 +1500,12 @@ Proof.
   inv H10. exploit deref_loc_receptive; eauto. intros [EQ [v1' A]]. subst t0.
   destruct (sem_binary_operation op v1' (typeof l) v2 (typeof r) m) as [v3'|] eqn:?.
   destruct (sem_cast v3' tyres (typeof l)) as [v4'|] eqn:?.
-  destruct (classic (exists t2', exists m'', assign_loc (Genv.globalenv p) (typeof l) m b ofs v4' t2' m'')).
-  destruct H1 as [t2' [m'' P]]. 
+  destruct (classic (exists t2', exists m'', exists sq'',
+    assign_loc (Genv.globalenv p) (typeof l) m sq b ofs v4' t2' m'' sq'')).
+  destruct H1 as [t2' [m'' [sq'' P]]]. 
   econstructor; econstructor. left; eapply step_assignop with (v1 := v1'); eauto. simpl; reflexivity. 
   econstructor; econstructor. left; eapply step_assignop_stuck with (v1 := v1'); eauto. 
-  rewrite Heqo; rewrite Heqo0. intros; red; intros; elim H1. exists t0; exists m'0; auto.
+  rewrite Heqo; rewrite Heqo0. intros; red; intros; elim H1. exists t0; exists m'0; exists sq'0; auto.
   econstructor; econstructor. left; eapply step_assignop_stuck with (v1 := v1'); eauto. 
   rewrite Heqo; rewrite Heqo0; auto.
   econstructor; econstructor. left; eapply step_assignop_stuck with (v1 := v1'); eauto. 
@@ -1507,11 +1514,12 @@ Proof.
   exploit deref_loc_receptive; eauto. intros [EQ [v1' A]]. subst t1.
   destruct (sem_binary_operation op v1' (typeof l) v2 (typeof r) m) as [v3'|] eqn:?.
   destruct (sem_cast v3' tyres (typeof l)) as [v4'|] eqn:?.
-  destruct (classic (exists t2', exists m'', assign_loc (Genv.globalenv p) (typeof l) m b ofs v4' t2' m'')).
-  destruct H1 as [t2' [m'' P]]. 
+  destruct (classic (exists t2', exists m'', exists sq'',
+    assign_loc (Genv.globalenv p) (typeof l) m sq b ofs v4' t2' m'' sq'')).
+  destruct H1 as [t2' [m'' [sq'' P]]]. 
   econstructor; econstructor. left; eapply step_assignop with (v1 := v1'); eauto. simpl; reflexivity. 
   econstructor; econstructor. left; eapply step_assignop_stuck with (v1 := v1'); eauto. 
-  rewrite Heqo; rewrite Heqo0. intros; red; intros; elim H1. exists t2; exists m'; auto.
+  rewrite Heqo; rewrite Heqo0. intros; red; intros; elim H1. exists t2; exists m'; exists sq'; auto.
   econstructor; econstructor. left; eapply step_assignop_stuck with (v1 := v1'); eauto. 
   rewrite Heqo; rewrite Heqo0; auto.
   econstructor; econstructor. left; eapply step_assignop_stuck with (v1 := v1'); eauto. 
@@ -1523,11 +1531,12 @@ Proof.
   inv H9. exploit deref_loc_receptive; eauto. intros [EQ [v1' A]]. subst t0.
   destruct (sem_incrdecr id v1' (typeof l)) as [v2'|] eqn:?.
   destruct (sem_cast v2' (typeconv (typeof l)) (typeof l)) as [v3'|] eqn:?.
-  destruct (classic (exists t2', exists m'', assign_loc (Genv.globalenv p) (typeof l) m b ofs v3' t2' m'')).
-  destruct H1 as [t2' [m'' P]]. 
+  destruct (classic (exists t2', exists m'', exists sq'',
+    assign_loc (Genv.globalenv p) (typeof l) m sq b ofs v3' t2' m'' sq'')).
+  destruct H1 as [t2' [m'' [sq'' P]]]. 
   econstructor; econstructor. left; eapply step_postincr with (v1 := v1'); eauto. simpl; reflexivity. 
   econstructor; econstructor. left; eapply step_postincr_stuck with (v1 := v1'); eauto. 
-  rewrite Heqo; rewrite Heqo0. intros; red; intros; elim H1. exists t0; exists m'0; auto.
+  rewrite Heqo; rewrite Heqo0. intros; red; intros; elim H1. exists t0; exists m'0; exists sq'0; auto.
   econstructor; econstructor. left; eapply step_postincr_stuck with (v1 := v1'); eauto. 
   rewrite Heqo; rewrite Heqo0; auto.
   econstructor; econstructor. left; eapply step_postincr_stuck with (v1 := v1'); eauto. 
@@ -1536,11 +1545,12 @@ Proof.
   exploit deref_loc_receptive; eauto. intros [EQ [v1' A]]. subst t1.
   destruct (sem_incrdecr id v1' (typeof l)) as [v2'|] eqn:?.
   destruct (sem_cast v2' (typeconv (typeof l)) (typeof l)) as [v3'|] eqn:?.
-  destruct (classic (exists t2', exists m'', assign_loc (Genv.globalenv p) (typeof l) m b ofs v3' t2' m'')).
-  destruct H1 as [t2' [m'' P]]. 
+  destruct (classic (exists t2', exists m'', exists sq'',
+    assign_loc (Genv.globalenv p) (typeof l) m sq b ofs v3' t2' m'' sq'')).
+  destruct H1 as [t2' [m'' [sq'' P]]]. 
   econstructor; econstructor. left; eapply step_postincr with (v1 := v1'); eauto. simpl; reflexivity. 
   econstructor; econstructor. left; eapply step_postincr_stuck with (v1 := v1'); eauto. 
-  rewrite Heqo; rewrite Heqo0. intros; red; intros; elim H1. exists t2; exists m'; auto.
+  rewrite Heqo; rewrite Heqo0. intros; red; intros; elim H1. exists t2; exists m'; exists sq'; auto.
   econstructor; econstructor. left; eapply step_postincr_stuck with (v1 := v1'); eauto. 
   rewrite Heqo; rewrite Heqo0; auto.
   econstructor; econstructor. left; eapply step_postincr_stuck with (v1 := v1'); eauto. 
@@ -1649,128 +1659,142 @@ Definition outcome_result_value (out: outcome) (t: type) (v: val) : Prop :=
   memory state, and [t] the trace of input/output events performed
   during this evaluation.  *)
 
-Inductive eval_expression: env -> mem -> expr -> trace -> mem -> val -> Prop :=
-  | eval_expression_intro: forall e m a t m' a' v,
-      eval_expr e m RV a t m' a' -> eval_simple_rvalue ge e m' a' v ->
-      eval_expression e m a t m' v
+Inductive eval_expression: env -> mem -> seqs -> expr -> trace -> mem -> seqs -> val -> Prop :=
+  | eval_expression_intro: forall e m sq a t m' sq' a' v,
+      eval_expr e m sq RV a t m' sq' a' ->
+      eval_simple_rvalue ge e m' sq' a' v ->
+      eval_expression e m sq a t m' sq' v
 
-with eval_expr: env -> mem -> kind -> expr -> trace -> mem -> expr -> Prop :=
-  | eval_val: forall e m v ty,
-      eval_expr e m RV (Eval v ty) E0 m (Eval v ty)
-  | eval_var: forall e m x ty,
-      eval_expr e m LV (Evar x ty) E0 m (Evar x ty)
-  | eval_field: forall e m a t m' a' f ty,
-      eval_expr e m RV a t m' a' ->
-      eval_expr e m LV (Efield a f ty) t m' (Efield a' f ty)
-  | eval_valof: forall e m a t m' a' ty,
+with eval_expr: env -> mem -> seqs -> kind -> expr -> trace -> mem -> seqs -> expr -> Prop :=
+  | eval_val: forall e m sq v ty,
+      eval_expr e m sq RV (Eval v ty) E0 m sq (Eval v ty)
+  | eval_var: forall e m sq x ty,
+      eval_expr e m sq LV (Evar x ty) E0 m sq (Evar x ty)
+  | eval_field: forall e m sq a t m' sq' a' f ty,
+      eval_expr e m sq RV a t m' sq' a' ->
+      eval_expr e m sq LV (Efield a f ty) t m' sq' (Efield a' f ty)
+  | eval_valof: forall e m sq a t m' sq' a' ty,
       type_is_volatile (typeof a) = false ->
-      eval_expr e m LV a t m' a' ->
-      eval_expr e m RV (Evalof a ty) t m' (Evalof a' ty)
-  | eval_valof_volatile: forall e m a t1 m' a' ty b ofs t2 v,
+      eval_expr e m sq LV a t m' sq' a' ->
+      eval_expr e m sq RV (Evalof a ty) t m' sq' (Evalof a' ty)
+  | eval_valof_volatile: forall e m sq a t1 m' sq' a' ty b ofs t2 v,
       type_is_volatile (typeof a) = true ->
-      eval_expr e m LV a t1 m' a' ->
-      eval_simple_lvalue ge e m' a' b ofs ->
-      deref_loc ge (typeof a) m' b ofs t2 v ->
+      eval_expr e m sq LV a t1 m' sq' a' ->
+      eval_simple_lvalue ge e m' sq' a' b ofs ->
+      deref_loc ge (typeof a) m' sq' b ofs t2 v ->
       ty = typeof a ->
-      eval_expr e m RV (Evalof a ty) (t1 ** t2) m' (Eval v ty)
-  | eval_deref: forall e m a t m' a' ty,
-      eval_expr e m RV a t m' a' ->
-      eval_expr e m LV (Ederef a ty) t m' (Ederef a' ty)
-  | eval_addrof: forall e m a t m' a' ty,
-      eval_expr e m LV a t m' a' ->
-      eval_expr e m RV (Eaddrof a ty) t m' (Eaddrof a' ty)
-  | eval_unop: forall e m a t m' a' op ty,
-      eval_expr e m RV a t m' a' ->
-      eval_expr e m RV (Eunop op a ty) t m' (Eunop op a' ty)
-  | eval_binop: forall e m a1 t1 m' a1' a2 t2 m'' a2' op ty,
-      eval_expr e m RV a1 t1 m' a1' -> eval_expr e m' RV a2 t2 m'' a2' ->
-      eval_expr e m RV (Ebinop op a1 a2 ty) (t1 ** t2) m'' (Ebinop op a1' a2' ty)
-  | eval_cast: forall e m a t m' a' ty,
-      eval_expr e m RV a t m' a' ->
-      eval_expr e m RV (Ecast a ty) t m' (Ecast a' ty)
-  | eval_seqand_true: forall e m a1 a2 ty t1 m' a1' v1 t2 m'' a2' v2 v' v,
-      eval_expr e m RV a1 t1 m' a1' -> eval_simple_rvalue ge e m' a1' v1 ->
+      eval_expr e m sq RV (Evalof a ty) (t1 ** t2) m' sq' (Eval v ty)
+  | eval_deref: forall e m sq a t m' sq' a' ty,
+      eval_expr e m sq RV a t m' sq' a' ->
+      eval_expr e m sq LV (Ederef a ty) t m' sq' (Ederef a' ty)
+  | eval_addrof: forall e m sq a t m' sq' a' ty,
+      eval_expr e m sq LV a t m' sq' a' ->
+      eval_expr e m sq RV (Eaddrof a ty) t m' sq' (Eaddrof a' ty)
+  | eval_unop: forall e m sq a t m' sq' a' op ty,
+      eval_expr e m sq RV a t m' sq' a' ->
+      eval_expr e m sq RV (Eunop op a ty) t m' sq' (Eunop op a' ty)
+  | eval_binop: forall e m sq a1 t1 m' sq' a1' a2 t2 m'' sq'' a2' op ty,
+      eval_expr e m sq RV a1 t1 m' sq' a1' ->
+      eval_expr e m' sq' RV a2 t2 m'' sq'' a2' ->
+      eval_expr e m sq RV (Ebinop op a1 a2 ty) (t1 ** t2) m'' sq'' (Ebinop op a1' a2' ty)
+  | eval_cast: forall e m sq a t m' sq' a' ty,
+      eval_expr e m sq RV a t m' sq' a' ->
+      eval_expr e m sq RV (Ecast a ty) t m' sq' (Ecast a' ty)
+  | eval_seqand_true: forall e m sq a1 a2 ty t1 m' sq' a1' v1 t2 m'' sq'' a2' v2 v' v,
+      eval_expr e m sq RV a1 t1 m' sq' a1' ->
+      eval_simple_rvalue ge e m' sq' a1' v1 ->
       bool_val v1 (typeof a1) = Some true ->
-      eval_expr e m' RV a2 t2 m'' a2' -> eval_simple_rvalue ge e m'' a2' v2 ->
+      eval_expr e m' empty_seqs RV a2 t2 m'' sq'' a2' ->
+      eval_simple_rvalue ge e m'' sq'' a2' v2 ->
       sem_cast v2 (typeof a2) type_bool = Some v' ->
       sem_cast v' type_bool ty = Some v ->
-      eval_expr e m RV (Eseqand a1 a2 ty) (t1**t2) m'' (Eval v ty)
-  | eval_seqand_false: forall e m a1 a2 ty t1 m' a1' v1,
-      eval_expr e m RV a1 t1 m' a1' -> eval_simple_rvalue ge e m' a1' v1 ->
+      eval_expr e m sq RV (Eseqand a1 a2 ty) (t1**t2) m'' sq'' (Eval v ty)
+  | eval_seqand_false: forall e m sq a1 a2 ty t1 m' sq' a1' v1,
+      eval_expr e m sq RV a1 t1 m' sq' a1' ->
+      eval_simple_rvalue ge e m' sq' a1' v1 ->
       bool_val v1 (typeof a1) = Some false ->
-      eval_expr e m RV (Eseqand a1 a2 ty) t1 m' (Eval (Vint Int.zero) ty)
-  | eval_seqor_false: forall e m a1 a2 ty t1 m' a1' v1 t2 m'' a2' v2 v' v,
-      eval_expr e m RV a1 t1 m' a1' -> eval_simple_rvalue ge e m' a1' v1 ->
+      eval_expr e m sq RV (Eseqand a1 a2 ty) t1 m' sq' (Eval (Vint Int.zero) ty)
+  | eval_seqor_false: forall e m sq a1 a2 ty t1 m' sq' a1' v1 t2 m'' sq'' a2' v2 v' v,
+      eval_expr e m sq RV a1 t1 m' sq' a1' ->
+      eval_simple_rvalue ge e m' sq' a1' v1 ->
       bool_val v1 (typeof a1) = Some false ->
-      eval_expr e m' RV a2 t2 m'' a2' -> eval_simple_rvalue ge e m'' a2' v2 ->
+      eval_expr e m' empty_seqs RV a2 t2 m'' sq'' a2' ->
+      eval_simple_rvalue ge e m'' sq'' a2' v2 ->
       sem_cast v2 (typeof a2) type_bool = Some v' ->
       sem_cast v' type_bool ty = Some v ->
-      eval_expr e m RV (Eseqor a1 a2 ty) (t1**t2) m'' (Eval v ty)
-  | eval_seqor_true: forall e m a1 a2 ty t1 m' a1' v1,
-      eval_expr e m RV a1 t1 m' a1' -> eval_simple_rvalue ge e m' a1' v1 ->
+      eval_expr e m sq RV (Eseqor a1 a2 ty) (t1**t2) m'' sq'' (Eval v ty)
+  | eval_seqor_true: forall e m sq a1 a2 ty t1 m' sq' a1' v1,
+      eval_expr e m sq RV a1 t1 m' sq' a1' ->
+      eval_simple_rvalue ge e m' sq' a1' v1 ->
       bool_val v1 (typeof a1) = Some true ->
-      eval_expr e m RV (Eseqor a1 a2 ty) t1 m' (Eval (Vint Int.one) ty)
-  | eval_condition: forall e m a1 a2 a3 ty t1 m' a1' v1 t2 m'' a' v' b v,
-      eval_expr e m RV a1 t1 m' a1' -> eval_simple_rvalue ge e m' a1' v1 ->
+      eval_expr e m sq RV (Eseqor a1 a2 ty) t1 m' sq' (Eval (Vint Int.one) ty)
+  | eval_condition: forall e m sq a1 a2 a3 ty t1 m' sq' a1' v1 t2 m'' sq'' a' v' b v,
+      eval_expr e m sq RV a1 t1 m' sq' a1' ->
+      eval_simple_rvalue ge e m' sq' a1' v1 ->
       bool_val v1 (typeof a1) = Some b ->
-      eval_expr e m' RV (if b then a2 else a3) t2 m'' a' -> eval_simple_rvalue ge e m'' a' v' ->
+      eval_expr e m' empty_seqs RV (if b then a2 else a3) t2 m'' sq'' a' ->
+      eval_simple_rvalue ge e m'' sq'' a' v' ->
       sem_cast v' (typeof (if b then a2 else a3)) ty = Some v ->
-      eval_expr e m RV (Econdition a1 a2 a3 ty) (t1**t2) m'' (Eval v ty)
-  | eval_sizeof: forall e m ty' ty,
-      eval_expr e m RV (Esizeof ty' ty) E0 m (Esizeof ty' ty)
-  | eval_alignof: forall e m ty' ty,
-      eval_expr e m RV (Ealignof ty' ty) E0 m (Ealignof ty' ty)
-  | eval_assign: forall e m l r ty t1 m1 l' t2 m2 r' b ofs v v' t3 m3,
-      eval_expr e m LV l t1 m1 l' -> eval_expr e m1 RV r t2 m2 r' ->
-      eval_simple_lvalue ge e m2 l' b ofs ->
-      eval_simple_rvalue ge e m2 r' v ->
+      eval_expr e m sq RV (Econdition a1 a2 a3 ty) (t1**t2) m'' sq'' (Eval v ty)
+  | eval_sizeof: forall e m sq ty' ty,
+      eval_expr e m sq RV (Esizeof ty' ty) E0 m sq (Esizeof ty' ty)
+  | eval_alignof: forall e m sq ty' ty,
+      eval_expr e m sq RV (Ealignof ty' ty) E0 m sq (Ealignof ty' ty)
+  | eval_assign: forall e m sq l r ty t1 m1 sq1 l' t2 m2 sq2 r' b ofs v v' t3 m3 sq3,
+      eval_expr e m sq LV l t1 m1 sq1 l' ->
+      eval_expr e m1 sq1 RV r t2 m2 sq2 r' ->
+      eval_simple_lvalue ge e m2 sq2 l' b ofs ->
+      eval_simple_rvalue ge e m2 sq2 r' v ->
       sem_cast v (typeof r) (typeof l) = Some v' ->
-      assign_loc ge (typeof l) m2 b ofs v' t3 m3 ->
+      assign_loc ge (typeof l) m2 sq2 b ofs v' t3 m3 sq3 ->
       ty = typeof l ->
-      eval_expr e m RV (Eassign l r ty) (t1**t2**t3) m3 (Eval v' ty)
-  | eval_assignop: forall e m op l r tyres ty t1 m1 l' t2 m2 r' b ofs
-                          v1 v2 v3 v4 t3 t4 m3,
-      eval_expr e m LV l t1 m1 l' -> eval_expr e m1 RV r t2 m2 r' ->
-      eval_simple_lvalue ge e m2 l' b ofs ->
-      deref_loc ge (typeof l) m2 b ofs t3 v1 ->
-      eval_simple_rvalue ge e m2 r' v2 ->
+      eval_expr e m sq RV (Eassign l r ty) (t1**t2**t3) m3 sq3 (Eval v' ty)
+  | eval_assignop: forall e m sq op l r tyres ty t1 m1 sq1 l' t2 m2 sq2 r' b ofs
+                          v1 v2 v3 v4 t3 t4 m3 sq3,
+      eval_expr e m sq LV l t1 m1 sq1 l' ->
+      eval_expr e m1 sq1 RV r t2 m2 sq2 r' ->
+      eval_simple_lvalue ge e m2 sq2 l' b ofs ->
+      deref_loc ge (typeof l) m2 sq2 b ofs t3 v1 ->
+      eval_simple_rvalue ge e m2 sq2 r' v2 ->
       sem_binary_operation op v1 (typeof l) v2 (typeof r) m2 = Some v3 ->
       sem_cast v3 tyres (typeof l) = Some v4 ->
-      assign_loc ge (typeof l) m2 b ofs v4 t4 m3 ->
+      assign_loc ge (typeof l) m2 sq2 b ofs v4 t4 m3 sq3 ->
       ty = typeof l ->
-      eval_expr e m RV (Eassignop op l r tyres ty) (t1**t2**t3**t4) m3 (Eval v4 ty)
-  | eval_postincr: forall e m id l ty t1 m1 l' b ofs v1 v2 v3 m2 t2 t3,
-      eval_expr e m LV l t1 m1 l' ->
-      eval_simple_lvalue ge e m1 l' b ofs ->
-      deref_loc ge ty m1 b ofs t2 v1 ->
+      eval_expr e m sq RV (Eassignop op l r tyres ty) (t1**t2**t3**t4) m3 sq3 (Eval v4 ty)
+  | eval_postincr: forall e m sq id l ty t1 m1 sq1 l' b ofs v1 v2 v3 m2 sq2 t2 t3,
+      eval_expr e m sq LV l t1 m1 sq1 l' ->
+      eval_simple_lvalue ge e m1 sq1 l' b ofs ->
+      deref_loc ge ty m1 sq1 b ofs t2 v1 ->
       sem_incrdecr id v1 ty = Some v2 ->
       sem_cast v2 (typeconv ty) ty = Some v3 ->
-      assign_loc ge ty m1 b ofs v3 t3 m2 ->
+      assign_loc ge ty m1 sq1 b ofs v3 t3 m2 sq2 ->
       ty = typeof l ->
-      eval_expr e m RV (Epostincr id l ty) (t1**t2**t3) m2 (Eval v1 ty)
-  | eval_comma: forall e m r1 r2 ty t1 m1 r1' v1 t2 m2 r2',
-      eval_expr e m RV r1 t1 m1 r1' ->
-      eval_simple_rvalue ge e m1 r1' v1 ->
-      eval_expr e m1 RV r2 t2 m2 r2' ->
+      eval_expr e m sq RV (Epostincr id l ty) (t1**t2**t3) m2 sq2 (Eval v1 ty)
+  | eval_comma: forall (sp : bool) e m sq r1 r2 ty t1 m1 sq1 r1' v1 t2 m2 sq2 r2',
+      eval_expr e m sq RV r1 t1 m1 sq1 r1' ->
+      eval_simple_rvalue ge e m1 sq1 r1' v1 ->
+      eval_expr e m1 (if sp then empty_seqs else sq1) RV r2 t2 m2 sq2 r2' ->
       ty = typeof r2 ->
-      eval_expr e m RV (Ecomma r1 r2 ty) (t1**t2) m2 r2'
-  | eval_call: forall e m rf rargs ty t1 m1 rf' t2 m2 rargs' vf vargs
+      eval_expr e m sq RV (Ecomma sp r1 r2 ty) (t1**t2) m2 sq2 r2'
+
+  | eval_call: forall e m sq rf rargs ty t1 m1 sq1 rf' t2 m2 sq2 rargs' vf vargs
                       targs tres cconv fd t3 m3 vres,
-      eval_expr e m RV rf t1 m1 rf' -> eval_exprlist e m1 rargs t2 m2 rargs' ->
-      eval_simple_rvalue ge e m2 rf' vf ->
-      eval_simple_list ge e m2 rargs' targs vargs ->
+      eval_expr e m sq RV rf t1 m1 sq1 rf' -> eval_exprlist e m1 sq1 rargs t2 m2 sq2 rargs' ->
+      eval_simple_rvalue ge e m2 sq2 rf' vf ->
+      eval_simple_list ge e m2 sq2 rargs' targs vargs ->
       classify_fun (typeof rf) = fun_case_f targs tres cconv ->
       Genv.find_funct ge vf = Some fd ->
       type_of_fundef fd = Tfunction targs tres cconv ->
       eval_funcall m2 fd vargs t3 m3 vres ->
-      eval_expr e m RV (Ecall rf rargs ty) (t1**t2**t3) m3 (Eval vres ty)
+      eval_expr e m sq RV (Ecall rf rargs ty) (t1**t2**t3) m3 empty_seqs (Eval vres ty)
 
-with eval_exprlist: env -> mem -> exprlist -> trace -> mem -> exprlist -> Prop :=
-  | eval_nil: forall e m,
-      eval_exprlist e m Enil E0 m Enil
-  | eval_cons: forall e m a1 al t1 m1 a1' t2 m2 al',
-      eval_expr e m RV a1 t1 m1 a1' -> eval_exprlist e m1 al t2 m2 al' ->
-      eval_exprlist e m (Econs a1 al) (t1**t2) m2 (Econs a1' al')
+with eval_exprlist: env -> mem -> seqs -> exprlist -> trace -> mem -> seqs -> exprlist -> Prop :=
+  | eval_nil: forall e m sq,
+      eval_exprlist e m sq Enil E0 m sq Enil
+  | eval_cons: forall e m sq a1 al t1 m1 sq1 a1' t2 m2 sq2 al',
+      eval_expr e m sq RV a1 t1 m1 sq1 a1' ->
+      eval_exprlist e m1 sq1 al t2 m2 sq2 al' ->
+      eval_exprlist e m sq (Econs a1 al) (t1**t2) m2 sq2 (Econs a1' al')
 
 (** [exec_stmt ge e m1 s t m2 out] describes the execution of 
   the statement [s].  [out] is the outcome for this execution.
@@ -1782,8 +1806,8 @@ with exec_stmt: env -> mem -> statement -> trace -> mem -> outcome -> Prop :=
   | exec_Sskip:   forall e m,
       exec_stmt e m Sskip
                E0 m Out_normal
-  | exec_Sdo:     forall e m a t m' v,
-      eval_expression e m a t m' v ->
+  | exec_Sdo:     forall e m a t m' sq' v,
+      eval_expression e m empty_seqs a t m' sq' v ->
       exec_stmt e m (Sdo a)
                 t m' Out_normal
   | exec_Sseq_1:   forall e m s1 s2 t1 m1 t2 m2 out,
@@ -1796,8 +1820,8 @@ with exec_stmt: env -> mem -> statement -> trace -> mem -> outcome -> Prop :=
       out <> Out_normal ->
       exec_stmt e m (Ssequence s1 s2)
                 t1 m1 out
-  | exec_Sifthenelse: forall e m a s1 s2 t1 m1 v1 t2 m2 b out,
-      eval_expression e m a t1 m1 v1 ->
+  | exec_Sifthenelse: forall e m a s1 s2 t1 m1 sq1 v1 t2 m2 b out,
+      eval_expression e m empty_seqs a t1 m1 sq1 v1 ->
       bool_val v1 (typeof a) = Some b ->
       exec_stmt e m1 (if b then s1 else s2) t2 m2 out ->
       exec_stmt e m (Sifthenelse a s1 s2)
@@ -1805,8 +1829,8 @@ with exec_stmt: env -> mem -> statement -> trace -> mem -> outcome -> Prop :=
   | exec_Sreturn_none:   forall e m,
       exec_stmt e m (Sreturn None)
                E0 m (Out_return None)
-  | exec_Sreturn_some: forall e m a t m' v,
-      eval_expression e m a t m' v ->
+  | exec_Sreturn_some: forall e m a t m' sq' v,
+      eval_expression e m empty_seqs a t m' sq' v ->
       exec_stmt e m (Sreturn (Some a))
                 t m' (Out_return (Some(v, typeof a)))
   | exec_Sbreak:   forall e m,
@@ -1815,30 +1839,30 @@ with exec_stmt: env -> mem -> statement -> trace -> mem -> outcome -> Prop :=
   | exec_Scontinue:   forall e m,
       exec_stmt e m Scontinue
                E0 m Out_continue
-  | exec_Swhile_false: forall e m a s t m' v,
-      eval_expression e m a t m' v ->
+  | exec_Swhile_false: forall e m a s t m' sq' v,
+      eval_expression e m empty_seqs a t m' sq' v ->
       bool_val v (typeof a) = Some false ->
       exec_stmt e m (Swhile a s)
                 t m' Out_normal
-  | exec_Swhile_stop: forall e m a s t1 m1 v t2 m2 out' out,
-      eval_expression e m a t1 m1 v ->
+  | exec_Swhile_stop: forall e m a s t1 m1 sq1 v t2 m2 out' out,
+      eval_expression e m empty_seqs a t1 m1 sq1 v ->
       bool_val v (typeof a) = Some true ->
       exec_stmt e m1 s t2 m2 out' ->
       out_break_or_return out' out ->
       exec_stmt e m (Swhile a s)
                 (t1**t2) m2 out
-  | exec_Swhile_loop: forall e m a s t1 m1 v t2 m2 out1 t3 m3 out,
-      eval_expression e m a t1 m1 v ->
+  | exec_Swhile_loop: forall e m a s t1 m1 sq1 v t2 m2 out1 t3 m3 out,
+      eval_expression e m empty_seqs a t1 m1 sq1 v ->
       bool_val v (typeof a) = Some true ->
       exec_stmt e m1 s t2 m2 out1 ->
       out_normal_or_continue out1 ->
       exec_stmt e m2 (Swhile a s) t3 m3 out ->
       exec_stmt e m (Swhile a s)
                 (t1 ** t2 ** t3) m3 out
-  | exec_Sdowhile_false: forall e m s a t1 m1 out1 t2 m2 v,
+  | exec_Sdowhile_false: forall e m s a t1 m1 out1 t2 m2 sq2 v,
       exec_stmt e m s t1 m1 out1 ->
       out_normal_or_continue out1 ->
-      eval_expression e m1 a t2 m2 v ->
+      eval_expression e m1 empty_seqs a t2 m2 sq2 v ->
       bool_val v (typeof a) = Some false ->
       exec_stmt e m (Sdowhile a s)
                 (t1 ** t2) m2 Out_normal
@@ -1847,10 +1871,10 @@ with exec_stmt: env -> mem -> statement -> trace -> mem -> outcome -> Prop :=
       out_break_or_return out1 out ->
       exec_stmt e m (Sdowhile a s)
                 t m1 out
-  | exec_Sdowhile_loop: forall e m s a t1 m1 out1 t2 m2 v t3 m3 out,
+  | exec_Sdowhile_loop: forall e m s a t1 m1 out1 t2 m2 sq2 v t3 m3 out,
       exec_stmt e m s t1 m1 out1 ->
       out_normal_or_continue out1 ->
-      eval_expression e m1 a t2 m2 v ->
+      eval_expression e m1 empty_seqs a t2 m2 sq2 v ->
       bool_val v (typeof a) = Some true ->
       exec_stmt e m2 (Sdowhile a s) t3 m3 out ->
       exec_stmt e m (Sdowhile a s) 
@@ -1860,20 +1884,20 @@ with exec_stmt: env -> mem -> statement -> trace -> mem -> outcome -> Prop :=
       exec_stmt e m1 (Sfor Sskip a2 a3 s) t2 m2 out ->
       exec_stmt e m (Sfor a1 a2 a3 s) 
                 (t1 ** t2) m2 out
-  | exec_Sfor_false: forall e m s a2 a3 t m' v,
-      eval_expression e m a2 t m' v ->
+  | exec_Sfor_false: forall e m s a2 a3 t m' sq' v,
+      eval_expression e m empty_seqs a2 t m' sq' v ->
       bool_val v (typeof a2) = Some false ->
       exec_stmt e m (Sfor Sskip a2 a3 s)
                 t m' Out_normal
-  | exec_Sfor_stop: forall e m s a2 a3 t1 m1 v t2 m2 out1 out,
-      eval_expression e m a2 t1 m1 v ->
+  | exec_Sfor_stop: forall e m s a2 a3 t1 m1 sq1 v t2 m2 out1 out,
+      eval_expression e m empty_seqs a2 t1 m1 sq1 v ->
       bool_val v (typeof a2) = Some true ->
       exec_stmt e m1 s t2 m2 out1 ->
       out_break_or_return out1 out ->
       exec_stmt e m (Sfor Sskip a2 a3 s)
                 (t1 ** t2) m2 out
-  | exec_Sfor_loop: forall e m s a2 a3 t1 m1 v t2 m2 out1 t3 m3 t4 m4 out,
-      eval_expression e m a2 t1 m1 v ->
+  | exec_Sfor_loop: forall e m s a2 a3 t1 m1 sq1 v t2 m2 out1 t3 m3 t4 m4 out,
+      eval_expression e m empty_seqs a2 t1 m1 sq1 v ->
       bool_val v (typeof a2) = Some true ->
       exec_stmt e m1 s t2 m2 out1 ->
       out_normal_or_continue out1 ->
@@ -1881,8 +1905,8 @@ with exec_stmt: env -> mem -> statement -> trace -> mem -> outcome -> Prop :=
       exec_stmt e m3 (Sfor Sskip a2 a3 s) t4 m4 out ->
       exec_stmt e m (Sfor Sskip a2 a3 s)
                 (t1 ** t2 ** t3 ** t4) m4 out
-  | exec_Sswitch:   forall e m a sl t1 m1 n t2 m2 out,
-      eval_expression e m a t1 m1 (Vint n) ->
+  | exec_Sswitch:   forall e m a sl t1 m1 sq1 n t2 m2 out,
+      eval_expression e m empty_seqs a t1 m1 sq1 (Vint n) ->
       exec_stmt e m1 (seq_of_labeled_statement (select_switch n sl)) t2 m2 out ->
       exec_stmt e m (Sswitch a sl)
                 (t1 ** t2) m2 (outcome_switch out)
@@ -1918,110 +1942,118 @@ Combined Scheme bigstep_induction from
   diverges in initial state [m1].  [T] is the trace of input/output
   events performed during this evaluation.  *)
 
-CoInductive evalinf_expr: env -> mem -> kind -> expr -> traceinf -> Prop :=
-  | evalinf_field: forall e m a t f ty,
-      evalinf_expr e m RV a t ->
-      evalinf_expr e m LV (Efield a f ty) t
-  | evalinf_valof: forall e m a t ty,
-      evalinf_expr e m LV a t ->
-      evalinf_expr e m RV (Evalof a ty) t
-  | evalinf_deref: forall e m a t ty,
-      evalinf_expr e m RV a t ->
-      evalinf_expr e m LV (Ederef a ty) t
-  | evalinf_addrof: forall e m a t ty,
-      evalinf_expr e m LV a t ->
-      evalinf_expr e m RV (Eaddrof a ty) t
-  | evalinf_unop: forall e m a t op ty,
-      evalinf_expr e m RV a t ->
-      evalinf_expr e m RV (Eunop op a ty) t
-  | evalinf_binop_left: forall e m a1 t1 a2 op ty,
-      evalinf_expr e m RV a1 t1 ->
-      evalinf_expr e m RV (Ebinop op a1 a2 ty) t1
-  | evalinf_binop_right: forall e m a1 t1 m' a1' a2 t2 op ty,
-      eval_expr e m RV a1 t1 m' a1' -> evalinf_expr e m' RV a2 t2 ->
-      evalinf_expr e m RV (Ebinop op a1 a2 ty) (t1 *** t2)
-  | evalinf_cast: forall e m a t ty,
-      evalinf_expr e m RV a t ->
-      evalinf_expr e m RV (Ecast a ty) t
-  | evalinf_seqand: forall e m a1 a2 ty t1,
-      evalinf_expr e m RV a1 t1 ->
-      evalinf_expr e m RV (Eseqand a1 a2 ty) t1
-  | evalinf_seqand_2: forall e m a1 a2 ty t1 m' a1' v1 t2,
-      eval_expr e m RV a1 t1 m' a1' -> eval_simple_rvalue ge e m' a1' v1 ->
+CoInductive evalinf_expr: env -> mem -> seqs -> kind -> expr -> traceinf -> Prop :=
+  | evalinf_field: forall e m sq a t f ty,
+      evalinf_expr e m sq RV a t ->
+      evalinf_expr e m sq LV (Efield a f ty) t
+  | evalinf_valof: forall e m sq a t ty,
+      evalinf_expr e m sq LV a t ->
+      evalinf_expr e m sq RV (Evalof a ty) t
+  | evalinf_deref: forall e m sq a t ty,
+      evalinf_expr e m sq RV a t ->
+      evalinf_expr e m sq LV (Ederef a ty) t
+  | evalinf_addrof: forall e m sq a t ty,
+      evalinf_expr e m sq LV a t ->
+      evalinf_expr e m sq RV (Eaddrof a ty) t
+  | evalinf_unop: forall e m sq a t op ty,
+      evalinf_expr e m sq RV a t ->
+      evalinf_expr e m sq RV (Eunop op a ty) t
+  | evalinf_binop_left: forall e m sq a1 t1 a2 op ty,
+      evalinf_expr e m sq RV a1 t1 ->
+      evalinf_expr e m sq RV (Ebinop op a1 a2 ty) t1
+  | evalinf_binop_right: forall e m sq a1 t1 m' sq' a1' a2 t2 op ty,
+      eval_expr e m sq RV a1 t1 m' sq' a1' ->
+      evalinf_expr e m' sq' RV a2 t2 ->
+      evalinf_expr e m sq RV (Ebinop op a1 a2 ty) (t1 *** t2)
+  | evalinf_cast: forall e m sq a t ty,
+      evalinf_expr e m sq RV a t ->
+      evalinf_expr e m sq RV (Ecast a ty) t
+  | evalinf_seqand: forall e m sq a1 a2 ty t1,
+      evalinf_expr e m sq RV a1 t1 ->
+      evalinf_expr e m sq RV (Eseqand a1 a2 ty) t1
+  | evalinf_seqand_2: forall e m sq a1 a2 ty t1 m' sq' a1' v1 t2,
+      eval_expr e m sq RV a1 t1 m' sq' a1' ->
+      eval_simple_rvalue ge e m' sq' a1' v1 ->
       bool_val v1 (typeof a1) = Some true ->
-      evalinf_expr e m' RV a2 t2 ->
-      evalinf_expr e m RV (Eseqand a1 a2 ty) (t1***t2)
-  | evalinf_seqor: forall e m a1 a2 ty t1,
-      evalinf_expr e m RV a1 t1 ->
-      evalinf_expr e m RV (Eseqor a1 a2 ty) t1
-  | evalinf_seqor_2: forall e m a1 a2 ty t1 m' a1' v1 t2,
-      eval_expr e m RV a1 t1 m' a1' -> eval_simple_rvalue ge e m' a1' v1 ->
+      evalinf_expr e m' empty_seqs RV a2 t2 ->
+      evalinf_expr e m sq RV (Eseqand a1 a2 ty) (t1***t2)
+  | evalinf_seqor: forall e m sq a1 a2 ty t1,
+      evalinf_expr e m sq RV a1 t1 ->
+      evalinf_expr e m sq RV (Eseqor a1 a2 ty) t1
+  | evalinf_seqor_2: forall e m sq a1 a2 ty t1 m' sq' a1' v1 t2,
+      eval_expr e m sq RV a1 t1 m' sq' a1' ->
+      eval_simple_rvalue ge e m' sq' a1' v1 ->
       bool_val v1 (typeof a1) = Some false ->
-      evalinf_expr e m' RV a2 t2 ->
-      evalinf_expr e m RV (Eseqor a1 a2 ty) (t1***t2)
-  | evalinf_condition: forall e m a1 a2 a3 ty t1,
-      evalinf_expr e m RV a1 t1 ->
-      evalinf_expr e m RV (Econdition a1 a2 a3 ty) t1
-  | evalinf_condition_2: forall e m a1 a2 a3 ty t1 m' a1' v1 t2 b,
-      eval_expr e m RV a1 t1 m' a1' -> eval_simple_rvalue ge e m' a1' v1 ->
+      evalinf_expr e m' empty_seqs RV a2 t2 ->
+      evalinf_expr e m sq RV (Eseqor a1 a2 ty) (t1***t2)
+  | evalinf_condition: forall e m sq a1 a2 a3 ty t1,
+      evalinf_expr e m sq RV a1 t1 ->
+      evalinf_expr e m sq RV (Econdition a1 a2 a3 ty) t1
+  | evalinf_condition_2: forall e m sq a1 a2 a3 ty t1 m' sq' a1' v1 t2 b,
+      eval_expr e m sq RV a1 t1 m' sq' a1' ->
+      eval_simple_rvalue ge e m' sq' a1' v1 ->
       bool_val v1 (typeof a1) = Some b ->
-      evalinf_expr e m' RV (if b then a2 else a3) t2 ->
-      evalinf_expr e m RV (Econdition a1 a2 a3 ty) (t1***t2)
-  | evalinf_assign_left: forall e m a1 t1 a2 ty,
-      evalinf_expr e m LV a1 t1 ->
-      evalinf_expr e m RV (Eassign a1 a2 ty) t1
-  | evalinf_assign_right: forall e m a1 t1 m' a1' a2 t2 ty,
-      eval_expr e m LV a1 t1 m' a1' -> evalinf_expr e m' RV a2 t2 ->
-      evalinf_expr e m RV (Eassign a1 a2 ty) (t1 *** t2)
-  | evalinf_assignop_left: forall e m a1 t1 a2 op tyres ty,
-      evalinf_expr e m LV a1 t1 ->
-      evalinf_expr e m RV (Eassignop op a1 a2 tyres ty) t1
-  | evalinf_assignop_right: forall e m a1 t1 m' a1' a2 t2 op tyres ty,
-      eval_expr e m LV a1 t1 m' a1' -> evalinf_expr e m' RV a2 t2 ->
-      evalinf_expr e m RV (Eassignop op a1 a2 tyres ty) (t1 *** t2)
-  | evalinf_postincr: forall e m a t id ty,
-      evalinf_expr e m LV a t ->
-      evalinf_expr e m RV (Epostincr id a ty) t
-  | evalinf_comma_left: forall e m a1 t1 a2 ty,
-      evalinf_expr e m RV a1 t1 ->
-      evalinf_expr e m RV (Ecomma a1 a2 ty) t1
-  | evalinf_comma_right: forall e m a1 t1 m1 a1' v1 a2 t2 ty,
-      eval_expr e m RV a1 t1 m1 a1' -> eval_simple_rvalue ge e m1 a1' v1 ->
+      evalinf_expr e m' empty_seqs RV (if b then a2 else a3) t2 ->
+      evalinf_expr e m sq RV (Econdition a1 a2 a3 ty) (t1***t2)
+  | evalinf_assign_left: forall e m sq a1 t1 a2 ty,
+      evalinf_expr e m sq LV a1 t1 ->
+      evalinf_expr e m sq RV (Eassign a1 a2 ty) t1
+  | evalinf_assign_right: forall e m sq a1 t1 m' sq' a1' a2 t2 ty,
+      eval_expr e m sq LV a1 t1 m' sq' a1' ->
+      evalinf_expr e m' sq' RV a2 t2 ->
+      evalinf_expr e m sq RV (Eassign a1 a2 ty) (t1 *** t2)
+  | evalinf_assignop_left: forall e m sq a1 t1 a2 op tyres ty,
+      evalinf_expr e m sq LV a1 t1 ->
+      evalinf_expr e m sq RV (Eassignop op a1 a2 tyres ty) t1
+  | evalinf_assignop_right: forall e m sq a1 t1 m' sq' a1' a2 t2 op tyres ty,
+      eval_expr e m sq LV a1 t1 m' sq' a1' ->
+      evalinf_expr e m' sq' RV a2 t2 ->
+      evalinf_expr e m sq RV (Eassignop op a1 a2 tyres ty) (t1 *** t2)
+  | evalinf_postincr: forall e m sq a t id ty,
+      evalinf_expr e m sq LV a t ->
+      evalinf_expr e m sq RV (Epostincr id a ty) t
+  | evalinf_comma_left: forall sp e m sq a1 t1 a2 ty,
+      evalinf_expr e m sq RV a1 t1 ->
+      evalinf_expr e m sq RV (Ecomma sp a1 a2 ty) t1
+  | evalinf_comma_right: forall (sp : bool) e m sq a1 t1 m1 sq1 a1' v1 a2 t2 ty,
+      eval_expr e m sq RV a1 t1 m1 sq1 a1' ->
+      eval_simple_rvalue ge e m1 sq1 a1' v1 ->
       ty = typeof a2 ->
-      evalinf_expr e m1 RV a2 t2 ->
-      evalinf_expr e m RV (Ecomma a1 a2 ty) (t1 *** t2)
-  | evalinf_call_left: forall e m a1 t1 a2 ty,
-      evalinf_expr e m RV a1 t1 ->
-      evalinf_expr e m RV (Ecall a1 a2 ty) t1
-  | evalinf_call_right: forall e m a1 t1 m1 a1' a2 t2 ty,
-      eval_expr e m RV a1 t1 m1 a1' -> 
-      evalinf_exprlist e m1 a2 t2 ->
-      evalinf_expr e m RV (Ecall a1 a2 ty) (t1 *** t2)
-  | evalinf_call: forall e m rf rargs ty t1 m1 rf' t2 m2 rargs' vf vargs
+      evalinf_expr e m1 (if sp then empty_seqs else sq1) RV a2 t2 ->
+      evalinf_expr e m sq RV (Ecomma sp a1 a2 ty) (t1 *** t2)
+  | evalinf_call_left: forall e m sq a1 t1 a2 ty,
+      evalinf_expr e m sq RV a1 t1 ->
+      evalinf_expr e m sq RV (Ecall a1 a2 ty) t1
+  | evalinf_call_right: forall e m sq a1 t1 m1 sq1 a1' a2 t2 ty,
+      eval_expr e m sq RV a1 t1 m1 sq1 a1' -> 
+      evalinf_exprlist e m1 sq1 a2 t2 ->
+      evalinf_expr e m sq RV (Ecall a1 a2 ty) (t1 *** t2)
+  | evalinf_call: forall e m sq rf rargs ty t1 m1 sq1 rf' t2 m2 sq2 rargs' vf vargs
                       targs tres cconv fd t3,
-      eval_expr e m RV rf t1 m1 rf' -> eval_exprlist e m1 rargs t2 m2 rargs' ->
-      eval_simple_rvalue ge e m2 rf' vf ->
-      eval_simple_list ge e m2 rargs' targs vargs ->
+      eval_expr e m sq RV rf t1 m1 sq1 rf' -> eval_exprlist e m1 sq1 rargs t2 m2 sq2 rargs' ->
+      eval_simple_rvalue ge e m2 sq2 rf' vf ->
+      eval_simple_list ge e m2 sq2 rargs' targs vargs ->
       classify_fun (typeof rf) = fun_case_f targs tres cconv ->
       Genv.find_funct ge vf = Some fd ->
       type_of_fundef fd = Tfunction targs tres cconv ->
       evalinf_funcall m2 fd vargs t3 ->
-      evalinf_expr e m RV (Ecall rf rargs ty) (t1***t2***t3)
+      evalinf_expr e m sq RV (Ecall rf rargs ty) (t1***t2***t3)
 
-with evalinf_exprlist: env -> mem -> exprlist -> traceinf -> Prop :=
-  | evalinf_cons_left: forall e m a1 al t1,
-      evalinf_expr e m RV a1 t1 ->
-      evalinf_exprlist e m (Econs a1 al) t1
-  | evalinf_cons_right: forall e m a1 al t1 m1 a1' t2,
-      eval_expr e m RV a1 t1 m1 a1' -> evalinf_exprlist e m1 al t2 ->
-      evalinf_exprlist e m (Econs a1 al) (t1***t2)
+with evalinf_exprlist: env -> mem -> seqs -> exprlist -> traceinf -> Prop :=
+  | evalinf_cons_left: forall e m sq a1 al t1,
+      evalinf_expr e m sq RV a1 t1 ->
+      evalinf_exprlist e m sq (Econs a1 al) t1
+  | evalinf_cons_right: forall e m sq a1 al t1 m1 sq1 a1' t2,
+      eval_expr e m sq RV a1 t1 m1 sq1 a1' ->
+      evalinf_exprlist e m1 sq1 al t2 ->
+      evalinf_exprlist e m sq (Econs a1 al) (t1***t2)
 
 (** [execinf_stmt ge e m1 s t] describes the diverging execution of 
   the statement [s].  *)
 
 with execinf_stmt: env -> mem -> statement -> traceinf -> Prop :=
   | execinf_Sdo:     forall e m a t,
-      evalinf_expr e m RV a t ->
+      evalinf_expr e m empty_seqs RV a t ->
       execinf_stmt e m (Sdo a) t
   | execinf_Sseq_1:   forall e m s1 s2 t1,
       execinf_stmt e m s1 t1 ->
@@ -2031,26 +2063,26 @@ with execinf_stmt: env -> mem -> statement -> traceinf -> Prop :=
       execinf_stmt e m1 s2 t2 ->
       execinf_stmt e m (Ssequence s1 s2) (t1***t2)
   | execinf_Sifthenelse_test: forall e m a s1 s2 t1,
-      evalinf_expr e m RV a t1 ->
+      evalinf_expr e m empty_seqs RV a t1 ->
       execinf_stmt e m (Sifthenelse a s1 s2) t1
-  | execinf_Sifthenelse: forall e m a s1 s2 t1 m1 v1 t2 b,
-      eval_expression e m a t1 m1 v1 ->
+  | execinf_Sifthenelse: forall e m a s1 s2 t1 m1 sq1 v1 t2 b,
+      eval_expression e m empty_seqs a t1 m1 sq1 v1 ->
       bool_val v1 (typeof a) = Some b ->
       execinf_stmt e m1 (if b then s1 else s2) t2 ->
       execinf_stmt e m (Sifthenelse a s1 s2) (t1***t2)
   | execinf_Sreturn_some: forall e m a t,
-      evalinf_expr e m RV a t ->
+      evalinf_expr e m empty_seqs RV a t ->
       execinf_stmt e m (Sreturn (Some a)) t
   | execinf_Swhile_test: forall e m a s t1,
-      evalinf_expr e m RV a t1 ->
+      evalinf_expr e m empty_seqs RV a t1 ->
       execinf_stmt e m (Swhile a s) t1
-  | execinf_Swhile_body: forall e m a s t1 m1 v t2,
-      eval_expression e m a t1 m1 v ->
+  | execinf_Swhile_body: forall e m a s t1 m1 sq1 v t2,
+      eval_expression e m empty_seqs a t1 m1 sq1 v ->
       bool_val v (typeof a) = Some true ->
       execinf_stmt e m1 s t2 ->
       execinf_stmt e m (Swhile a s) (t1***t2)
-  | execinf_Swhile_loop: forall e m a s t1 m1 v t2 m2 out1 t3,
-      eval_expression e m a t1 m1 v ->
+  | execinf_Swhile_loop: forall e m a s t1 m1 sq1 v t2 m2 out1 t3,
+      eval_expression e m empty_seqs a t1 m1 sq1 v ->
       bool_val v (typeof a) = Some true ->
       exec_stmt e m1 s t2 m2 out1 ->
       out_normal_or_continue out1 ->
@@ -2062,12 +2094,12 @@ with execinf_stmt: env -> mem -> statement -> traceinf -> Prop :=
   | execinf_Sdowhile_test: forall e m s a t1 m1 out1 t2,
       exec_stmt e m s t1 m1 out1 ->
       out_normal_or_continue out1 ->
-      evalinf_expr e m1 RV a t2 ->
+      evalinf_expr e m1 empty_seqs RV a t2 ->
       execinf_stmt e m (Sdowhile a s) (t1***t2)
-  | execinf_Sdowhile_loop: forall e m s a t1 m1 out1 t2 m2 v t3,
+  | execinf_Sdowhile_loop: forall e m s a t1 m1 out1 t2 m2 sq2 v t3,
       exec_stmt e m s t1 m1 out1 ->
       out_normal_or_continue out1 ->
-      eval_expression e m1 a t2 m2 v ->
+      eval_expression e m1 empty_seqs a t2 m2 sq2 v ->
       bool_val v (typeof a) = Some true ->
       execinf_stmt e m2 (Sdowhile a s) t3 ->
       execinf_stmt e m (Sdowhile a s) (t1***t2***t3)
@@ -2079,22 +2111,22 @@ with execinf_stmt: env -> mem -> statement -> traceinf -> Prop :=
       execinf_stmt e m1 (Sfor Sskip a2 a3 s) t2 ->
       execinf_stmt e m (Sfor a1 a2 a3 s) (t1***t2)
   | execinf_Sfor_test: forall e m s a2 a3 t,
-      evalinf_expr e m RV a2 t ->
+      evalinf_expr e m empty_seqs RV a2 t ->
       execinf_stmt e m (Sfor Sskip a2 a3 s) t
-  | execinf_Sfor_body: forall e m s a2 a3 t1 m1 v t2,
-      eval_expression e m a2 t1 m1 v ->
+  | execinf_Sfor_body: forall e m s a2 a3 t1 m1 sq1 v t2,
+      eval_expression e m empty_seqs a2 t1 m1 sq1 v ->
       bool_val v (typeof a2) = Some true ->
       execinf_stmt e m1 s t2 ->
       execinf_stmt e m (Sfor Sskip a2 a3 s) (t1***t2)
-  | execinf_Sfor_next: forall e m s a2 a3 t1 m1 v t2 m2 out1 t3,
-      eval_expression e m a2 t1 m1 v ->
+  | execinf_Sfor_next: forall e m s a2 a3 t1 m1 sq1 v t2 m2 out1 t3,
+      eval_expression e m empty_seqs a2 t1 m1 sq1 v ->
       bool_val v (typeof a2) = Some true ->
       exec_stmt e m1 s t2 m2 out1 ->
       out_normal_or_continue out1 ->
       execinf_stmt e m2 a3 t3 ->
       execinf_stmt e m (Sfor Sskip a2 a3 s) (t1***t2***t3)
-  | execinf_Sfor_loop: forall e m s a2 a3 t1 m1 v t2 m2 out1 t3 m3 t4,
-      eval_expression e m a2 t1 m1 v ->
+  | execinf_Sfor_loop: forall e m s a2 a3 t1 m1 sq1 v t2 m2 out1 t3 m3 t4,
+      eval_expression e m empty_seqs a2 t1 m1 sq1 v ->
       bool_val v (typeof a2) = Some true ->
       exec_stmt e m1 s t2 m2 out1 ->
       out_normal_or_continue out1 ->
@@ -2102,10 +2134,10 @@ with execinf_stmt: env -> mem -> statement -> traceinf -> Prop :=
       execinf_stmt e m3 (Sfor Sskip a2 a3 s) t4 ->
       execinf_stmt e m (Sfor Sskip a2 a3 s) (t1***t2***t3***t4)
   | execinf_Sswitch_expr:   forall e m a sl t1,
-      evalinf_expr e m RV a t1 ->
+      evalinf_expr e m empty_seqs RV a t1 ->
       execinf_stmt e m (Sswitch a sl) t1
-  | execinf_Sswitch_body:   forall e m a sl t1 m1 n t2,
-      eval_expression e m a t1 m1 (Vint n) ->
+  | execinf_Sswitch_body:   forall e m a sl t1 m1 sq1 n t2,
+      eval_expression e m empty_seqs a t1 m1 sq1 (Vint n) ->
       execinf_stmt e m1 (seq_of_labeled_statement (select_switch n sl)) t2 ->
       execinf_stmt e m (Sswitch a sl) (t1***t2)
 
@@ -2134,10 +2166,10 @@ Inductive outcome_state_match
       call_cont k' = call_cont k ->
       outcome_state_match e m f k 
         (Out_return None) (State f (Sreturn None) k' e m)
-  | osm_return_some: forall v ty k',
+  | osm_return_some: forall v ty k' sq,
       call_cont k' = call_cont k ->
       outcome_state_match e m f k
-        (Out_return (Some (v, ty))) (ExprState f (Eval v ty) (Kreturn k') e m).
+        (Out_return (Some (v, ty))) (ExprState f (Eval v ty) (Kreturn k') e m sq).
 
 Lemma is_call_cont_call_cont:
   forall k, is_call_cont k -> call_cont k = k.
@@ -2176,21 +2208,21 @@ Proof.
 Qed.
 
 Lemma bigstep_to_steps:
-  (forall e m a t m' v,
-   eval_expression e m a t m' v ->
+  (forall e m sq a t m' sq' v,
+   eval_expression e m sq a t m' sq' v ->
    forall f k,
-   star step ge (ExprState f a k e m) t (ExprState f (Eval v (typeof a)) k e m'))
-/\(forall e m K a t m' a',
-   eval_expr e m K a t m' a' ->
+   star step ge (ExprState f a k e m sq) t (ExprState f (Eval v (typeof a)) k e m' sq'))
+/\(forall e m sq K a t m' sq' a',
+   eval_expr e m sq K a t m' sq' a' ->
    forall C f k, leftcontext K RV C ->
    simple a' = true /\ typeof a' = typeof a /\
-   star step ge (ExprState f (C a) k e m) t (ExprState f (C a') k e m'))
-/\(forall e m al t m' al',
-   eval_exprlist e m al t m' al' ->
+   star step ge (ExprState f (C a) k e m sq) t (ExprState f (C a') k e m' sq'))
+/\(forall e m sq al t m' sq' al',
+   eval_exprlist e m sq al t m' sq' al' ->
    forall a1 al2 ty C f k, leftcontext RV RV C -> simple a1 = true -> simplelist al2 = true ->
    simplelist al' = true /\
-   star step ge (ExprState f (C (Ecall a1 (exprlist_app al2 al) ty)) k e m)
-              t (ExprState f (C (Ecall a1 (exprlist_app al2 al') ty)) k e m'))
+   star step ge (ExprState f (C (Ecall a1 (exprlist_app al2 al) ty)) k e m sq)
+              t (ExprState f (C (Ecall a1 (exprlist_app al2 al') ty)) k e m' sq'))
 /\(forall e m s t m' out,
    exec_stmt e m s t m' out ->
    forall f k,
@@ -2206,7 +2238,7 @@ Proof.
 (* expression, general *)
   exploit (H0 (fun x => x) f k). constructor. intros [A [B C]].
   assert (match a' with Eval _ _ => False | _ => True end ->
-          star step ge (ExprState f a k e m) t (ExprState f (Eval v (typeof a)) k e m')).
+          star step ge (ExprState f a k e m sq) t (ExprState f (Eval v (typeof a)) k e m' sq')).
    intro. eapply star_right. eauto. left. eapply step_expr; eauto. traceEq. 
   destruct a'; auto.
   simpl in B. rewrite B in C. inv H1. auto. 
@@ -2271,7 +2303,7 @@ Proof.
   exploit (H0 (fun x => C(Eseqand x a2 ty))).
     eapply leftcontext_compose; eauto. repeat constructor. intros [A [B D]].
   simpl; intuition. eapply star_right. eexact D. 
-  left; eapply step_seqand_false; eauto. rewrite B; auto.
+  left. eapply step_seqand_false; eauto. rewrite B; auto.
   traceEq.
 (* seqor false *)
   exploit (H0 (fun x => C(Eseqor x a2 ty))).
@@ -2337,7 +2369,7 @@ Proof.
   left. eapply step_postincr; eauto. congruence. 
   traceEq.
 (* comma *)
-  exploit (H0 (fun x => C(Ecomma x r2 ty))).
+  exploit (H0 (fun x => C(Ecomma sp x r2 ty))).
     eapply leftcontext_compose; eauto. repeat constructor. intros [A [B D]].
   exploit (H3 C). auto. intros [E [F G]].
   simpl; intuition. congruence.
@@ -2620,27 +2652,27 @@ Proof.
 Qed.
 
 Lemma eval_expression_to_steps:
-   forall e m a t m' v,
-   eval_expression e m a t m' v ->
+   forall e m sq a t m' sq' v,
+   eval_expression e m sq a t m' sq' v ->
    forall f k,
-   star step ge (ExprState f a k e m) t (ExprState f (Eval v (typeof a)) k e m').
+   star step ge (ExprState f a k e m sq) t (ExprState f (Eval v (typeof a)) k e m' sq').
 Proof (proj1 bigstep_to_steps).
 
 Lemma eval_expr_to_steps:
-   forall e m K a t m' a',
-   eval_expr e m K a t m' a' ->
+   forall e m sq K a t m' sq' a',
+   eval_expr e m sq K a t m' sq' a' ->
    forall C f k, leftcontext K RV C ->
    simple a' = true /\ typeof a' = typeof a /\
-   star step ge (ExprState f (C a) k e m) t (ExprState f (C a') k e m').
+   star step ge (ExprState f (C a) k e m sq) t (ExprState f (C a') k e m' sq').
 Proof (proj1 (proj2 bigstep_to_steps)).
 
 Lemma eval_exprlist_to_steps:
-   forall e m al t m' al',
-   eval_exprlist e m al t m' al' ->
+   forall e m sq al t m' sq' al',
+   eval_exprlist e m sq al t m' sq' al' ->
    forall a1 al2 ty C f k, leftcontext RV RV C -> simple a1 = true -> simplelist al2 = true ->
    simplelist al' = true /\
-   star step ge (ExprState f (C (Ecall a1 (exprlist_app al2 al) ty)) k e m)
-              t (ExprState f (C (Ecall a1 (exprlist_app al2 al') ty)) k e m').
+   star step ge (ExprState f (C (Ecall a1 (exprlist_app al2 al) ty)) k e m sq)
+              t (ExprState f (C (Ecall a1 (exprlist_app al2 al') ty)) k e m' sq').
 Proof (proj1 (proj2 (proj2 bigstep_to_steps))).
 
 Lemma exec_stmt_to_steps:
@@ -2679,7 +2711,7 @@ Fixpoint esize (a: expr) : nat :=
   | Eassign l1 r2 _ => S(esize l1 + esize r2)%nat
   | Eassignop _ l1 r2 _ _ => S(esize l1 + esize r2)%nat
   | Epostincr _ l1 _ => S(esize l1)
-  | Ecomma r1 r2 _ => S(esize r1 + esize r2)%nat
+  | Ecomma _ r1 r2 _ => S(esize r1 + esize r2)%nat
   | Ecall r1 rl2 _ => S(esize r1 + esizelist rl2)%nat
   | Ebuiltin ef tyargs rl _ => S(esizelist rl)
   | Eparen r1 _ => S(esize r1)
@@ -2725,18 +2757,18 @@ Proof.
   cofix COS.
 
   assert (COE:
-    forall e m K a t C f k,
-    evalinf_expr e m K a t ->
+    forall e m sq K a t C f k,
+    evalinf_expr e m sq K a t ->
     leftcontext K RV C ->
-    forever_N step lt ge (esize a) (ExprState f (C a) k e m) t).
+    forever_N step lt ge (esize a) (ExprState f (C a) k e m sq) t).
   cofix COE.
 
   assert (COEL:
-    forall e m a t C f k a1 al ty,
-    evalinf_exprlist e m a t ->
+    forall e m sq a t C f k a1 al ty,
+    evalinf_exprlist e m sq a t ->
     leftcontext RV RV C -> simple a1 = true -> simplelist al = true ->
     forever_N step lt ge (esizelist a)
-                   (ExprState f (C (Ecall a1 (exprlist_app al a) ty)) k e m) t).
+                   (ExprState f (C (Ecall a1 (exprlist_app al a) ty)) k e m sq) t).
   cofix COEL.
   intros. inv H.
 (* cons left *)
@@ -2745,7 +2777,7 @@ Proof.
   eauto. eapply leftcontext_compose; eauto. constructor. auto. 
   apply exprlist_app_leftcontext; auto. traceEq.
 (* cons right *) 
-  destruct (eval_expr_to_steps _ _ _ _ _ _ _ H3 
+  destruct (eval_expr_to_steps _ _ _ _ _ _ _ _ _ H3 
              (fun x => C(Ecall a1 (exprlist_app al (Econs x al0)) ty)) f k)
   as [P [Q R]]. 
   eapply leftcontext_compose; eauto. repeat constructor. auto. 
@@ -2784,7 +2816,7 @@ Proof.
   eapply COE with (C := fun x => C(Ebinop op x a2 ty)). eauto. 
   eapply leftcontext_compose; eauto. repeat constructor. traceEq.
 (* binop right *)
-  destruct (eval_expr_to_steps _ _ _ _ _ _ _ H1 (fun x => C(Ebinop op x a2 ty)) f k)
+  destruct (eval_expr_to_steps _ _ _ _ _ _ _ _ _ H1 (fun x => C(Ebinop op x a2 ty)) f k)
   as [P [Q R]]. 
   eapply leftcontext_compose; eauto. repeat constructor.
   eapply forever_N_star with (a2 := (esize a2)). eexact R. simpl; omega.
@@ -2799,7 +2831,7 @@ Proof.
   eapply COE with (C := fun x => C(Eseqand x a2 ty)). eauto. 
   eapply leftcontext_compose; eauto. repeat constructor. traceEq.
 (* seqand 2 *)
-  destruct (eval_expr_to_steps _ _ _ _ _ _ _ H1 (fun x => C(Eseqand x a2 ty)) f k)
+  destruct (eval_expr_to_steps _ _ _ _ _ _ _ _ _ H1 (fun x => C(Eseqand x a2 ty)) f k)
   as [P [Q R]]. 
   eapply leftcontext_compose; eauto. repeat constructor.
   eapply forever_N_plus. eapply plus_right. eexact R. 
@@ -2812,7 +2844,7 @@ Proof.
   eapply COE with (C := fun x => C(Eseqor x a2 ty)). eauto. 
   eapply leftcontext_compose; eauto. repeat constructor. traceEq.
 (* seqor 2 *)
-  destruct (eval_expr_to_steps _ _ _ _ _ _ _ H1 (fun x => C(Eseqor x a2 ty)) f k)
+  destruct (eval_expr_to_steps _ _ _ _ _ _ _ _ _ H1 (fun x => C(Eseqor x a2 ty)) f k)
   as [P [Q R]]. 
   eapply leftcontext_compose; eauto. repeat constructor.
   eapply forever_N_plus. eapply plus_right. eexact R. 
@@ -2825,7 +2857,7 @@ Proof.
   eapply COE with (C := fun x => C(Econdition x a2 a3 ty)). eauto. 
   eapply leftcontext_compose; eauto. repeat constructor. traceEq.
 (* condition *)
-  destruct (eval_expr_to_steps _ _ _ _ _ _ _ H1 (fun x => C(Econdition x a2 a3 ty)) f k)
+  destruct (eval_expr_to_steps _ _ _ _ _ _ _ _ _ H1 (fun x => C(Econdition x a2 a3 ty)) f k)
   as [P [Q R]]. 
   eapply leftcontext_compose; eauto. repeat constructor.
   eapply forever_N_plus. eapply plus_right. eexact R. 
@@ -2838,7 +2870,7 @@ Proof.
   eapply COE with (C := fun x => C(Eassign x a2 ty)). eauto. 
   eapply leftcontext_compose; eauto. repeat constructor. traceEq.
 (* assign right *)
-  destruct (eval_expr_to_steps _ _ _ _ _ _ _ H1 (fun x => C(Eassign x a2 ty)) f k)
+  destruct (eval_expr_to_steps _ _ _ _ _ _ _ _ _ H1 (fun x => C(Eassign x a2 ty)) f k)
   as [P [Q R]]. 
   eapply leftcontext_compose; eauto. repeat constructor.
   eapply forever_N_star with (a2 := (esize a2)). eexact R. simpl; omega.
@@ -2849,7 +2881,7 @@ Proof.
   eapply COE with (C := fun x => C(Eassignop op x a2 tyres ty)). eauto. 
   eapply leftcontext_compose; eauto. repeat constructor. traceEq.
 (* assignop right *)
-  destruct (eval_expr_to_steps _ _ _ _ _ _ _ H1 (fun x => C(Eassignop op x a2 tyres ty)) f k)
+  destruct (eval_expr_to_steps _ _ _ _ _ _ _ _ _ H1 (fun x => C(Eassignop op x a2 tyres ty)) f k)
   as [P [Q R]]. 
   eapply leftcontext_compose; eauto. repeat constructor.
   eapply forever_N_star with (a2 := (esize a2)). eexact R. simpl; omega.
@@ -2861,10 +2893,10 @@ Proof.
   eapply leftcontext_compose; eauto. repeat constructor. traceEq.
 (* comma left *)
   eapply forever_N_star with (a2 := (esize a1)). apply star_refl. simpl; omega.
-  eapply COE with (C := fun x => C(Ecomma x a2 ty)). eauto. 
+  eapply COE with (C := fun x => C(Ecomma sp x a2 ty)). eauto. 
   eapply leftcontext_compose; eauto. repeat constructor. traceEq.
 (* comma right *)
-  destruct (eval_expr_to_steps _ _ _ _ _ _ _ H1 (fun x => C(Ecomma x a2 (typeof a2))) f k)
+  destruct (eval_expr_to_steps _ _ _ _ _ _ _ _ _ H1 (fun x => C(Ecomma sp x a2 (typeof a2))) f k)
   as [P [Q R]]. 
   eapply leftcontext_compose; eauto. repeat constructor.
   eapply forever_N_plus. eapply plus_right. eexact R. 
@@ -2875,16 +2907,16 @@ Proof.
   eapply COE with (C := fun x => C(Ecall x a2 ty)). eauto. 
   eapply leftcontext_compose; eauto. repeat constructor. traceEq.
 (* call right *)
-  destruct (eval_expr_to_steps _ _ _ _ _ _ _ H1 (fun x => C(Ecall x a2 ty)) f k)
+  destruct (eval_expr_to_steps _ _ _ _ _ _ _ _ _ H1 (fun x => C(Ecall x a2 ty)) f k)
   as [P [Q R]]. 
   eapply leftcontext_compose; eauto. repeat constructor.
   eapply forever_N_star with (a2 := (esizelist a2)). eexact R. simpl; omega.
   eapply COEL with (al := Enil). eauto. auto. auto. auto. traceEq.
 (* call *)
-  destruct (eval_expr_to_steps _ _ _ _ _ _ _ H1 (fun x => C(Ecall x rargs ty)) f k)
+  destruct (eval_expr_to_steps _ _ _ _ _ _ _ _ _ H1 (fun x => C(Ecall x rargs ty)) f k)
   as [P [Q R]]. 
   eapply leftcontext_compose; eauto. repeat constructor.
-  destruct (eval_exprlist_to_steps _ _ _ _ _ _ H2 rf' Enil ty C f k)
+  destruct (eval_exprlist_to_steps _ _ _ _ _ _ _ _ H2 rf' Enil ty C f k)
   as [S T]. auto. auto. simpl; auto.
   eapply forever_N_plus. eapply plus_right.
   eapply star_trans. eexact R. eexact T. reflexivity.
